Removed admits in TLSConstants, proved inversion lemmas

src/tls/TLSConstants.fst
@@ -4,7 +4,6 @@
    hash algorithm etc. *)
 module TLSConstants
 
-(* SMT solver parameters *)
 #set-options "--max_fuel 0 --initial_fuel 0 --max_ifuel 1 --initial_ifuel 1"
 
 open FStar.SeqProperties
@@ -15,45 +14,45 @@ open CoreCrypto
 
 (* Type representations for TLS negotiated values *)
 type protocolVersion =
-    | SSL_3p0 // supported, with no security guarantees
-    | TLS_1p0
-    | TLS_1p1
-    | TLS_1p2
-    | TLS_1p3
+  | SSL_3p0 // supported, with no security guarantees
+  | TLS_1p0
+  | TLS_1p1
+  | TLS_1p2
+  | TLS_1p3
 
 (* Key exchange algorithms *)
 type kexAlg =
-    | Kex_RSA
-    | Kex_DH
-    | Kex_DHE
-    | Kex_ECDHE
+  | Kex_RSA
+  | Kex_DH
+  | Kex_DHE
+  | Kex_ECDHE
 
 (* We retrieve cryptographic primitives from the CoreCrypto library *)
 type blockCipher = block_cipher
-type streamCipher = CoreCrypto.stream_cipher
-type aeadAlg = CoreCrypto.aead_cipher
+type streamCipher = stream_cipher
+type aeadAlg = aead_cipher
 
 type ivMode =
-    | Fresh
-    | Stale
+  | Fresh
+  | Stale
 
 type encAlg =
-    | Block of blockCipher
-    | Stream of streamCipher
+  | Block of blockCipher
+  | Stream of streamCipher
 
 type hashAlg =
-    | NULL
-    | MD5SHA1
-    | Hash of hash_alg (* Defined in CoreCrypto library *)
+  | NULL
+  | MD5SHA1
+  | Hash of hash_alg
 
 type macAlg =
-    | HMAC     of hash_alg
-    | SSLKHASH of hash_alg
+  | HMAC     of hash_alg
+  | SSLKHASH of hash_alg
 
 type aeAlg =
-    | MACOnly : hash_alg -> aeAlg
-    | MtE   : encAlg -> hash_alg -> aeAlg
-    | AEAD  : aeadAlg -> hash_alg -> aeAlg
+  | MACOnly: hash_alg -> aeAlg
+  | MtE: encAlg -> hash_alg -> aeAlg
+  | AEAD: aeadAlg -> hash_alg -> aeAlg
 
 // does this algorithm provide padding support with TLS 1.2? 
 let lhae = function
@@ -82,43 +81,42 @@ assume val strongAuthAE: pv:protocolVersion -> ae:aeAlg -> Lemma(strongAEAlg pv 
 
 type sigAlg = CoreCrypto.sig_alg
 
-type sigHashAlg = sigAlg * hashAlg
+(* This is the old version of the inverse predicate. According to CF,
+   verification was harder with this style, so we moved to the new style with
+   pinverse_t + lemmas. The type abbrevations lemma_inverse_* minimize the
+   syntactic overhead.
+
+  logic type pinverse (#a:Type) (#b:Type) (r:b -> b -> Type) (=f:a -> Tot b) =
+    y:b -> Tot (xopt:result a{(forall (x:a). r (f x) y <==> (xopt = Correct x))})
+*)
+
+type pinverse_t (#a:Type) (#b:Type) ($f:(a -> Tot b)) = b -> Tot (result a)
+
+inline type lemma_inverse_g_f (#a:Type) (#b:Type) ($f:a -> Tot b) ($g:b -> Tot (result a)) (x:a) =
+  g (f x) = Correct x
+
+inline type lemma_pinverse_f_g (#a:Type) (#b:Type) (r:b -> b -> Type) ($f:a -> Tot b) ($g:b -> Tot (result a)) (y:b) =
+  is_Correct (g y) ==> r (f (Correct._0 (g y))) y
 
 
 (* Serializing function for signature algorithms *)
 val sigAlgBytes: sigAlg -> Tot (lbytes 1)
 let sigAlgBytes sa =
-    match sa with
-    | CoreCrypto.RSASIG -> abyte 1z
-    | CoreCrypto.DSA    -> abyte 2z
-    | CoreCrypto.ECDSA  -> abyte 3z
-    | CoreCrypto.RSAPSS -> abyte 4z
-
-(* This is the old version of the inverse predicate. According to CF,
-   verification was harder with this style, so we moved to the new style with
-   pinverse_t + lemmas. The type abbrevations lemma_inverse_* minimize the
-   syntactic overhead. *)
-(* logic type pinverse (#a:Type) (#b:Type) (r:(b -> b -> Type)) (=f:(a -> Tot b)) =
-    (y:b -> Tot (xopt:result a{(forall (x:a). r (f x) y <==> (xopt = Correct x))})) *)
-
-type pinverse_t (#a:Type) (#b:Type) ($f:(a -> Tot b)) =
-    (y:b -> Tot (result a))
+  match sa with
+  | CoreCrypto.RSASIG -> abyte 1z
+  | CoreCrypto.DSA    -> abyte 2z
+  | CoreCrypto.ECDSA  -> abyte 3z
+  | CoreCrypto.RSAPSS -> abyte 4z
 
 (* Parsing function associated to sigAlgBytes *)
 val parseSigAlg: pinverse_t sigAlgBytes
 let parseSigAlg b =
-    match cbyte b with
-    | 1z -> Correct CoreCrypto.RSASIG
-    | 2z -> Correct CoreCrypto.DSA
-    | 3z -> Correct CoreCrypto.ECDSA
-    | 4z -> Correct CoreCrypto.RSAPSS
-    | _ -> Error (AD_decode_error, perror __SOURCE_FILE__ __LINE__ "")
-
-inline type lemma_inverse_g_f (#a:Type) (#b:Type) ($f:(a -> Tot b)) ($g:(b -> Tot (result a))) (x:a) = 
-  g (f x) = Correct x
-
-inline type lemma_pinverse_f_g (#a:Type) (#b:Type) (r:b -> b -> Type) ($f:(a -> Tot b)) ($g:(b -> Tot (result a))) (y:b) =
-  is_Correct (g y) ==> r (f (Correct._0 (g y))) y
+  match cbyte b with
+  | 1z -> Correct CoreCrypto.RSASIG
+  | 2z -> Correct CoreCrypto.DSA
+  | 3z -> Correct CoreCrypto.ECDSA
+  | 4z -> Correct CoreCrypto.RSAPSS
+  | _ -> Error (AD_decode_error, perror __SOURCE_FILE__ __LINE__ "")
 
 val inverse_sigAlg: x:_ -> Lemma
   (requires (True)) 
@@ -137,25 +135,25 @@ type hashAlg' = h:hashAlg{h <> NULL /\ h <> MD5SHA1 }
 
 #set-options "--max_fuel 0 --initial_fuel 0 --max_ifuel 2 --initial_ifuel 2"
 val hashAlgBytes: hashAlg' -> Tot (lbytes 1)
- let hashAlgBytes ha =
-   match ha with
-    | Hash MD5     -> abyte 1z
-    | Hash SHA1    -> abyte 2z
-    | Hash SHA224  -> abyte 3z
-    | Hash SHA256  -> abyte 4z
-    | Hash SHA384  -> abyte 5z
-    | Hash SHA512  -> abyte 6z
+let hashAlgBytes ha =
+  match ha with
+  | Hash MD5     -> abyte 1z
+  | Hash SHA1    -> abyte 2z
+  | Hash SHA224  -> abyte 3z
+  | Hash SHA256  -> abyte 4z
+  | Hash SHA384  -> abyte 5z
+  | Hash SHA512  -> abyte 6z
 
 val parseHashAlg: pinverse_t hashAlgBytes
 let parseHashAlg b =
-    match cbyte b with
-    | 1z -> Correct (Hash MD5)
-    | 2z -> Correct (Hash SHA1)
-    | 3z -> Correct (Hash SHA224)
-    | 4z -> Correct (Hash SHA256)
-    | 5z -> Correct (Hash SHA384)
-    | 6z -> Correct (Hash SHA512)
-    | _ -> Error (AD_decode_error, perror __SOURCE_FILE__ __LINE__ "")
+  match cbyte b with
+  | 1z -> Correct (Hash MD5)
+  | 2z -> Correct (Hash SHA1)
+  | 3z -> Correct (Hash SHA224)
+  | 4z -> Correct (Hash SHA256)
+  | 5z -> Correct (Hash SHA384)
+  | 6z -> Correct (Hash SHA512)
+  | _ -> Error (AD_decode_error, perror __SOURCE_FILE__ __LINE__ "")
 
 val inverse_hashAlg: x:_ -> Lemma
   (requires (True))
@@ -169,6 +167,7 @@ val pinverse_hashAlg: x:_ -> Lemma
   [SMTPat (hashAlgBytes (Correct._0 (parseHashAlg x)))]
 let pinverse_hashAlg x = ()
 
+
 let encKeySize = function
   | Stream RC4_128      -> 16
   | Block TDES_EDE_CBC  -> 24
@@ -178,7 +177,6 @@ let encKeySize = function
   | Block AES_128_CBC   -> 16
   | Block AES_256_CBC   -> 32
 
-// TODO: renamed from aeadIVSize to avoid clash with CoreCrypto
 let aeadSaltSize = function
   | AES_128_GCM -> 4
   | AES_256_GCM -> 4
@@ -201,75 +199,72 @@ let macSize = function
   | SSLKHASH alg -> hashSize (Hash alg)
 
 type scsv_suite =
-    | TLS_EMPTY_RENEGOTIATION_INFO_SCSV
+  | TLS_EMPTY_RENEGOTIATION_INFO_SCSV
 
 type cipherSuite =
-    | NullCipherSuite    : cipherSuite
-    | CipherSuite        : kexAlg -> option sig_alg -> aeAlg -> cipherSuite
-    | SCSV               : scsv_suite -> cipherSuite
+  | NullCipherSuite: cipherSuite
+  | CipherSuite    : kexAlg -> option sig_alg -> aeAlg -> cipherSuite
+  | SCSV           : scsv_suite -> cipherSuite
 
 type cipherSuites = list cipherSuite
 
 type compression =
-    | NullCompression
-    | UnknownCompression of byte
+  | NullCompression
+  | UnknownCompression of byte
 
 val compressionBytes: compression -> Tot (lbytes 1)
-let compressionBytes (comp:compression) =
-    match comp with
-    | NullCompression -> abyte 0z
-    | UnknownCompression b -> abyte b
+let compressionBytes comp =
+  match comp with
+  | NullCompression      -> abyte 0z
+  | UnknownCompression b -> abyte b
 
-val parseCompression: b:lbytes 1 -> Tot (cm:compression{Seq.equal (compressionBytes cm) b})
+// Not pinverse_t compressionBytes, because it never fails
+val parseCompression: b:lbytes 1
+  -> Tot (cm:compression{Seq.equal (compressionBytes cm) b})
 let parseCompression b =
-    match cbyte b with
-    | 0z -> NullCompression
-    | b  -> UnknownCompression b
+  match cbyte b with
+  | 0z -> NullCompression
+  | b  -> UnknownCompression b
 
 // We ignore compression methods we don't understand. This is a departure
 // from usual parsing, where we fail on unknown values, but that's how TLS
 // handles compression method lists.
 val parseCompressions: b:bytes -> Tot (list compression) (decreases (length b))
 let rec parseCompressions b =
-    let l = length b in
-    if l > 0
-    then
-        let (cmB,b) = split b 1 in
-        let cm = parseCompression cmB in
-        cm :: parseCompressions b
-    else []
+  if length b > 0
+  then
+    let cmB,b = split b 1 in
+    let cm = parseCompression cmB in
+    cm :: parseCompressions b
+  else []
 
-
-////////////////////////////////////////////////////////////////////////////////
-////////////////////////////////////////////////////////////////////////////////
-
-#set-options "--max_ifuel 4 --initial_ifuel 2 --max_fuel 2 --initial_fuel 2"
-
-val compressionMethodsBytes : cms:list compression -> Tot (lbytes (List.Tot.length cms))
+#set-options "--max_fuel 1 --initial_fuel 1 --max_ifuel 1 --initial_ifuel 1"
+val compressionMethodsBytes: cms:list compression
+  -> Tot (lbytes (List.Tot.length cms))
 let rec compressionMethodsBytes cms =
-   match cms with
-   | c::cs -> compressionBytes c @| compressionMethodsBytes cs
-   | []    -> empty_bytes
+  match cms with
+  | c::cs -> compressionBytes c @| compressionMethodsBytes cs
+  | []   -> empty_bytes
 
 #set-options "--max_fuel 0 --initial_fuel 0 --max_ifuel 1 --initial_ifuel 1"
-val versionBytes : protocolVersion -> Tot (lbytes 2)
+val versionBytes: protocolVersion -> Tot (lbytes 2)
 let versionBytes pv =
-    match pv with
-    | SSL_3p0 -> abyte2 ( 3z, 0z)
-    | TLS_1p0 -> abyte2 ( 3z, 1z)
-    | TLS_1p1 -> abyte2 ( 3z, 2z )
-    | TLS_1p2 -> abyte2 ( 3z, 3z )
-    | TLS_1p3 -> abyte2 ( 3z, 4z )
+  match pv with
+  | SSL_3p0 -> abyte2 ( 3z, 0z)
+  | TLS_1p0 -> abyte2 ( 3z, 1z)
+  | TLS_1p1 -> abyte2 ( 3z, 2z )
+  | TLS_1p2 -> abyte2 ( 3z, 3z )
+  | TLS_1p3 -> abyte2 ( 3z, 4z )
 
 val parseVersion: pinverse_t versionBytes
 let parseVersion v =
-    match cbyte2 v with
-    | ( 3z, 0z ) -> Correct(SSL_3p0)
-    | ( 3z, 1z ) -> Correct(TLS_1p0)
-    | ( 3z, 2z ) -> Correct(TLS_1p1)
-    | ( 3z, 3z ) -> Correct(TLS_1p2)
-    | ( 3z, 4z ) -> Correct(TLS_1p3)
-    | _ -> Error(AD_decode_error, perror __SOURCE_FILE__ __LINE__ "Parsed an unknown version")
+  match cbyte2 v with
+  | ( 3z, 0z ) -> Correct SSL_3p0
+  | ( 3z, 1z ) -> Correct TLS_1p0
+  | ( 3z, 2z ) -> Correct TLS_1p1
+  | ( 3z, 3z ) -> Correct TLS_1p2
+  | ( 3z, 4z ) -> Correct TLS_1p3
+  | _ -> Error(AD_decode_error, perror __SOURCE_FILE__ __LINE__ "Parsed an unknown version")
 
 val inverse_version: x:_ -> Lemma
   (requires (True))
@@ -284,26 +279,21 @@ val pinverse_version: x:_ -> Lemma
 let pinverse_version x = ()
 
 let minPV (a:protocolVersion) (b:protocolVersion) =
-  match (a,b) with
+  match a,b with
   | SSL_3p0, _  | _, SSL_3p0 -> SSL_3p0
   | TLS_1p0, _  | _, TLS_1p0 -> TLS_1p0
   | TLS_1p1, _  | _, TLS_1p1 -> TLS_1p1
   | TLS_1p2, _  | _, TLS_1p2 -> TLS_1p2
   | TLS_1p3, _  | _, TLS_1p3 -> TLS_1p3
 
-let somePV (a:protocolVersion) = Some a
 let geqPV a b = (b = minPV a b)
 
 
-let nullCipherSuite = NullCipherSuite
-
-let isNullCipherSuite cs = (cs = NullCipherSuite)
-
 val cipherSuiteBytesOpt: cipherSuite -> Tot (option (lbytes 2))
 let cipherSuiteBytesOpt cs =
-  let abyte2 b : option (lbytes 2) = Some (abyte2 b) in
+  let abyte2 b: option (lbytes 2) = Some (abyte2 b) in
     match cs with
-    | NullCipherSuite                                 -> abyte2 ( 0x00z, 0x00z )
+    | NullCipherSuite                                              -> abyte2 ( 0x00z, 0x00z )
 
     | CipherSuite Kex_RSA None (MACOnly MD5)                       -> abyte2 ( 0x00z, 0x01z )
     | CipherSuite Kex_RSA None (MACOnly SHA1)                      -> abyte2 ( 0x00z, 0x02z )
@@ -383,7 +373,9 @@ let cipherSuiteBytesOpt cs =
     | _ -> None
 
 let knownCipherSuite (c:cipherSuite) = is_Some (cipherSuiteBytesOpt c)
+
 type known_cipher_suite = c:cipherSuite{knownCipherSuite c}
+
 type known_cipher_suites = list known_cipher_suite
 
 val cipherSuiteBytes: known_cipher_suite -> Tot (lbytes 2)
@@ -391,100 +383,99 @@ let cipherSuiteBytes c = Some.v (cipherSuiteBytesOpt c)
 
 val parseCipherSuiteAux : lbytes 2 -> Tot (result cipherSuite)
 let parseCipherSuiteAux b =
-    match cbyte2 b with
-    | ( 0x00z, 0x00z ) -> Correct(NullCipherSuite)
+  match cbyte2 b with
+  | ( 0x00z, 0x00z ) -> Correct(NullCipherSuite)
 
-    | ( 0x00z, 0x01z ) -> Correct(CipherSuite Kex_RSA None (MACOnly MD5))
-    | ( 0x00z, 0x02z ) -> Correct(CipherSuite Kex_RSA None (MACOnly SHA1))
-    | ( 0x00z, 0x3Bz ) -> Correct(CipherSuite Kex_RSA None (MACOnly SHA256))
-    | ( 0x00z, 0x04z ) -> Correct(CipherSuite Kex_RSA None (MtE (Stream RC4_128) MD5))
-    | ( 0x00z, 0x05z ) -> Correct(CipherSuite Kex_RSA None (MtE (Stream RC4_128) SHA1))
+  | ( 0x00z, 0x01z ) -> Correct(CipherSuite Kex_RSA None (MACOnly MD5))
+  | ( 0x00z, 0x02z ) -> Correct(CipherSuite Kex_RSA None (MACOnly SHA1))
+  | ( 0x00z, 0x3Bz ) -> Correct(CipherSuite Kex_RSA None (MACOnly SHA256))
+  | ( 0x00z, 0x04z ) -> Correct(CipherSuite Kex_RSA None (MtE (Stream RC4_128) MD5))
+  | ( 0x00z, 0x05z ) -> Correct(CipherSuite Kex_RSA None (MtE (Stream RC4_128) SHA1))
 
-    | ( 0x00z, 0x0Az ) -> Correct(CipherSuite Kex_RSA None (MtE (Block TDES_EDE_CBC) SHA1))
-    | ( 0x00z, 0x2Fz ) -> Correct(CipherSuite Kex_RSA None (MtE (Block AES_128_CBC) SHA1))
-    | ( 0x00z, 0x35z ) -> Correct(CipherSuite Kex_RSA None (MtE (Block AES_256_CBC) SHA1))
-    | ( 0x00z, 0x3Cz ) -> Correct(CipherSuite Kex_RSA None (MtE (Block AES_128_CBC) SHA256))
-    | ( 0x00z, 0x3Dz ) -> Correct(CipherSuite Kex_RSA None (MtE (Block AES_256_CBC) SHA256))
+  | ( 0x00z, 0x0Az ) -> Correct(CipherSuite Kex_RSA None (MtE (Block TDES_EDE_CBC) SHA1))
+  | ( 0x00z, 0x2Fz ) -> Correct(CipherSuite Kex_RSA None (MtE (Block AES_128_CBC) SHA1))
+  | ( 0x00z, 0x35z ) -> Correct(CipherSuite Kex_RSA None (MtE (Block AES_256_CBC) SHA1))
+  | ( 0x00z, 0x3Cz ) -> Correct(CipherSuite Kex_RSA None (MtE (Block AES_128_CBC) SHA256))
+  | ( 0x00z, 0x3Dz ) -> Correct(CipherSuite Kex_RSA None (MtE (Block AES_256_CBC) SHA256))
 
-    (**************************************************************************)
-    | ( 0x00z, 0x0Dz ) -> Correct(CipherSuite Kex_DH (Some DSA) (MtE (Block TDES_EDE_CBC) SHA1))
-    | ( 0x00z, 0x10z ) -> Correct(CipherSuite Kex_DH (Some RSASIG) (MtE (Block TDES_EDE_CBC) SHA1))
-    | ( 0x00z, 0x13z ) -> Correct(CipherSuite Kex_DHE (Some DSA) (MtE (Block TDES_EDE_CBC) SHA1))
-    | ( 0x00z, 0x16z ) -> Correct(CipherSuite Kex_DHE (Some RSASIG) (MtE (Block TDES_EDE_CBC) SHA1))
+  (**************************************************************************)
+  | ( 0x00z, 0x0Dz ) -> Correct(CipherSuite Kex_DH (Some DSA) (MtE (Block TDES_EDE_CBC) SHA1))
+  | ( 0x00z, 0x10z ) -> Correct(CipherSuite Kex_DH (Some RSASIG) (MtE (Block TDES_EDE_CBC) SHA1))
+  | ( 0x00z, 0x13z ) -> Correct(CipherSuite Kex_DHE (Some DSA) (MtE (Block TDES_EDE_CBC) SHA1))
+  | ( 0x00z, 0x16z ) -> Correct(CipherSuite Kex_DHE (Some RSASIG) (MtE (Block TDES_EDE_CBC) SHA1))
 
-    | ( 0x00z, 0x30z ) -> Correct(CipherSuite Kex_DH (Some DSA) (MtE (Block AES_128_CBC) SHA1))
-    | ( 0x00z, 0x31z ) -> Correct(CipherSuite Kex_DH (Some RSASIG) (MtE (Block AES_128_CBC) SHA1))
-    | ( 0x00z, 0x32z ) -> Correct(CipherSuite Kex_DHE (Some DSA) (MtE (Block AES_128_CBC) SHA1))
-    | ( 0x00z, 0x33z ) -> Correct(CipherSuite Kex_DHE (Some RSASIG) (MtE (Block AES_128_CBC) SHA1))
+  | ( 0x00z, 0x30z ) -> Correct(CipherSuite Kex_DH (Some DSA) (MtE (Block AES_128_CBC) SHA1))
+  | ( 0x00z, 0x31z ) -> Correct(CipherSuite Kex_DH (Some RSASIG) (MtE (Block AES_128_CBC) SHA1))
+  | ( 0x00z, 0x32z ) -> Correct(CipherSuite Kex_DHE (Some DSA) (MtE (Block AES_128_CBC) SHA1))
+  | ( 0x00z, 0x33z ) -> Correct(CipherSuite Kex_DHE (Some RSASIG) (MtE (Block AES_128_CBC) SHA1))
 
-    | ( 0x00z, 0x36z ) -> Correct(CipherSuite Kex_DH (Some DSA) (MtE (Block AES_256_CBC) SHA1))
-    | ( 0x00z, 0x37z ) -> Correct(CipherSuite Kex_DH (Some RSASIG) (MtE (Block AES_256_CBC) SHA1))
-    | ( 0x00z, 0x38z ) -> Correct(CipherSuite Kex_DHE (Some DSA) (MtE (Block AES_256_CBC) SHA1))
-    | ( 0x00z, 0x39z ) -> Correct(CipherSuite Kex_DHE (Some RSASIG) (MtE (Block AES_256_CBC) SHA1))
+  | ( 0x00z, 0x36z ) -> Correct(CipherSuite Kex_DH (Some DSA) (MtE (Block AES_256_CBC) SHA1))
+  | ( 0x00z, 0x37z ) -> Correct(CipherSuite Kex_DH (Some RSASIG) (MtE (Block AES_256_CBC) SHA1))
+  | ( 0x00z, 0x38z ) -> Correct(CipherSuite Kex_DHE (Some DSA) (MtE (Block AES_256_CBC) SHA1))
+  | ( 0x00z, 0x39z ) -> Correct(CipherSuite Kex_DHE (Some RSASIG) (MtE (Block AES_256_CBC) SHA1))
 
-    | ( 0x00z, 0x3Ez ) -> Correct(CipherSuite Kex_DH (Some DSA) (MtE (Block AES_128_CBC) SHA256))
-    | ( 0x00z, 0x3Fz ) -> Correct(CipherSuite Kex_DH (Some RSASIG) (MtE (Block AES_128_CBC) SHA256))
-    | ( 0x00z, 0x40z ) -> Correct(CipherSuite Kex_DHE (Some DSA) (MtE (Block AES_128_CBC) SHA256))
-    | ( 0x00z, 0x67z ) -> Correct(CipherSuite Kex_DHE (Some RSASIG) (MtE (Block AES_128_CBC) SHA256))
+  | ( 0x00z, 0x3Ez ) -> Correct(CipherSuite Kex_DH (Some DSA) (MtE (Block AES_128_CBC) SHA256))
+  | ( 0x00z, 0x3Fz ) -> Correct(CipherSuite Kex_DH (Some RSASIG) (MtE (Block AES_128_CBC) SHA256))
+  | ( 0x00z, 0x40z ) -> Correct(CipherSuite Kex_DHE (Some DSA) (MtE (Block AES_128_CBC) SHA256))
+  | ( 0x00z, 0x67z ) -> Correct(CipherSuite Kex_DHE (Some RSASIG) (MtE (Block AES_128_CBC) SHA256))
 
-    | ( 0x00z, 0x68z ) -> Correct(CipherSuite Kex_DH (Some DSA) (MtE (Block AES_256_CBC) SHA256))
-    | ( 0x00z, 0x69z ) -> Correct(CipherSuite Kex_DH (Some RSASIG) (MtE (Block AES_256_CBC) SHA256))
-    | ( 0x00z, 0x6Az ) -> Correct(CipherSuite Kex_DHE (Some DSA) (MtE (Block AES_256_CBC) SHA256))
-    | ( 0x00z, 0x6Bz ) -> Correct(CipherSuite Kex_DHE (Some RSASIG) (MtE (Block AES_256_CBC) SHA256))
+  | ( 0x00z, 0x68z ) -> Correct(CipherSuite Kex_DH (Some DSA) (MtE (Block AES_256_CBC) SHA256))
+  | ( 0x00z, 0x69z ) -> Correct(CipherSuite Kex_DH (Some RSASIG) (MtE (Block AES_256_CBC) SHA256))
+  | ( 0x00z, 0x6Az ) -> Correct(CipherSuite Kex_DHE (Some DSA) (MtE (Block AES_256_CBC) SHA256))
+  | ( 0x00z, 0x6Bz ) -> Correct(CipherSuite Kex_DHE (Some RSASIG) (MtE (Block AES_256_CBC) SHA256))
 
-    (**************************************************************************)
-    | ( 0xc0z, 0x11z ) -> Correct(CipherSuite Kex_ECDHE (Some RSASIG) (MtE (Stream RC4_128) SHA1))
-    | ( 0xc0z, 0x12z ) -> Correct(CipherSuite Kex_ECDHE (Some RSASIG) (MtE (Block TDES_EDE_CBC) SHA1))
-    | ( 0xc0z, 0x13z ) -> Correct(CipherSuite Kex_ECDHE (Some RSASIG) (MtE (Block AES_128_CBC) SHA1))
-    | ( 0xc0z, 0x14z ) -> Correct(CipherSuite Kex_ECDHE (Some RSASIG) (MtE (Block AES_256_CBC) SHA1))
-    | ( 0xc0z, 0x27z ) -> Correct(CipherSuite Kex_ECDHE (Some RSASIG) (MtE (Block AES_128_CBC) SHA256))
-    | ( 0xc0z, 0x28z ) -> Correct(CipherSuite Kex_ECDHE (Some RSASIG) (MtE (Block AES_256_CBC) SHA384))
+  (**************************************************************************)
+  | ( 0xc0z, 0x11z ) -> Correct(CipherSuite Kex_ECDHE (Some RSASIG) (MtE (Stream RC4_128) SHA1))
+  | ( 0xc0z, 0x12z ) -> Correct(CipherSuite Kex_ECDHE (Some RSASIG) (MtE (Block TDES_EDE_CBC) SHA1))
+  | ( 0xc0z, 0x13z ) -> Correct(CipherSuite Kex_ECDHE (Some RSASIG) (MtE (Block AES_128_CBC) SHA1))
+  | ( 0xc0z, 0x14z ) -> Correct(CipherSuite Kex_ECDHE (Some RSASIG) (MtE (Block AES_256_CBC) SHA1))
+  | ( 0xc0z, 0x27z ) -> Correct(CipherSuite Kex_ECDHE (Some RSASIG) (MtE (Block AES_128_CBC) SHA256))
+  | ( 0xc0z, 0x28z ) -> Correct(CipherSuite Kex_ECDHE (Some RSASIG) (MtE (Block AES_256_CBC) SHA384))
 
-    | ( 0xc0z, 0x2fz ) -> Correct(CipherSuite Kex_ECDHE (Some RSASIG) (AEAD AES_128_GCM SHA256))
-    | ( 0xc0z, 0x30z ) -> Correct(CipherSuite Kex_ECDHE (Some RSASIG) (AEAD AES_256_GCM SHA384))
+  | ( 0xc0z, 0x2fz ) -> Correct(CipherSuite Kex_ECDHE (Some RSASIG) (AEAD AES_128_GCM SHA256))
+  | ( 0xc0z, 0x30z ) -> Correct(CipherSuite Kex_ECDHE (Some RSASIG) (AEAD AES_256_GCM SHA384))
 
-    (**************************************************************************)
-    | ( 0x00z, 0x18z ) -> Correct(CipherSuite Kex_DHE None (MtE (Stream RC4_128) MD5))
-    | ( 0x00z, 0x1Bz ) -> Correct(CipherSuite Kex_DHE None (MtE (Block TDES_EDE_CBC) SHA1))
-    | ( 0x00z, 0x34z ) -> Correct(CipherSuite Kex_DHE None (MtE (Block AES_128_CBC) SHA1))
-    | ( 0x00z, 0x3Az ) -> Correct(CipherSuite Kex_DHE None (MtE (Block AES_256_CBC) SHA1))
-    | ( 0x00z, 0x6Cz ) -> Correct(CipherSuite Kex_DHE None (MtE (Block AES_128_CBC) SHA256))
-    | ( 0x00z, 0x6Dz ) -> Correct(CipherSuite Kex_DHE None (MtE (Block AES_256_CBC) SHA256))
+  (**************************************************************************)
+  | ( 0x00z, 0x18z ) -> Correct(CipherSuite Kex_DHE None (MtE (Stream RC4_128) MD5))
+  | ( 0x00z, 0x1Bz ) -> Correct(CipherSuite Kex_DHE None (MtE (Block TDES_EDE_CBC) SHA1))
+  | ( 0x00z, 0x34z ) -> Correct(CipherSuite Kex_DHE None (MtE (Block AES_128_CBC) SHA1))
+  | ( 0x00z, 0x3Az ) -> Correct(CipherSuite Kex_DHE None (MtE (Block AES_256_CBC) SHA1))
+  | ( 0x00z, 0x6Cz ) -> Correct(CipherSuite Kex_DHE None (MtE (Block AES_128_CBC) SHA256))
+  | ( 0x00z, 0x6Dz ) -> Correct(CipherSuite Kex_DHE None (MtE (Block AES_256_CBC) SHA256))
 
-    (**************************************************************************)
-    | ( 0x00z, 0x9Cz ) -> Correct(CipherSuite Kex_RSA None     (AEAD AES_128_GCM SHA256))
-    | ( 0x00z, 0x9Dz ) -> Correct(CipherSuite Kex_RSA None     (AEAD AES_256_GCM SHA384))
+  (**************************************************************************)
+  | ( 0x00z, 0x9Cz ) -> Correct(CipherSuite Kex_RSA None	    (AEAD AES_128_GCM SHA256))
+  | ( 0x00z, 0x9Dz ) -> Correct(CipherSuite Kex_RSA None	    (AEAD AES_256_GCM SHA384))
 
-    | ( 0x00z, 0x9Ez ) -> Correct(CipherSuite Kex_DHE (Some RSASIG) (AEAD AES_128_GCM SHA256))
-    | ( 0x00z, 0x9Fz ) -> Correct(CipherSuite Kex_DHE (Some RSASIG) (AEAD AES_256_GCM SHA384))
-    | ( 0x00z, 0xA0z ) -> Correct(CipherSuite Kex_DH (Some RSASIG)  (AEAD AES_128_GCM SHA256))
-    | ( 0x00z, 0xA1z ) -> Correct(CipherSuite Kex_DH (Some RSASIG)  (AEAD AES_256_GCM SHA384))
+  | ( 0x00z, 0x9Ez ) -> Correct(CipherSuite Kex_DHE (Some RSASIG) (AEAD AES_128_GCM SHA256))
+  | ( 0x00z, 0x9Fz ) -> Correct(CipherSuite Kex_DHE (Some RSASIG) (AEAD AES_256_GCM SHA384))
+  | ( 0x00z, 0xA0z ) -> Correct(CipherSuite Kex_DH (Some RSASIG)  (AEAD AES_128_GCM SHA256))
+  | ( 0x00z, 0xA1z ) -> Correct(CipherSuite Kex_DH (Some RSASIG)  (AEAD AES_256_GCM SHA384))
 
-    | ( 0x00z, 0xA2z ) -> Correct(CipherSuite Kex_DHE (Some DSA) (AEAD AES_128_GCM SHA256))
-    | ( 0x00z, 0xA3z ) -> Correct(CipherSuite Kex_DHE (Some DSA) (AEAD AES_256_GCM SHA384))
-    | ( 0x00z, 0xA4z ) -> Correct(CipherSuite Kex_DH (Some DSA)  (AEAD AES_128_GCM SHA256))
-    | ( 0x00z, 0xA5z ) -> Correct(CipherSuite Kex_DH (Some DSA)  (AEAD AES_256_GCM SHA384))
+  | ( 0x00z, 0xA2z ) -> Correct(CipherSuite Kex_DHE (Some DSA) (AEAD AES_128_GCM SHA256))
+  | ( 0x00z, 0xA3z ) -> Correct(CipherSuite Kex_DHE (Some DSA) (AEAD AES_256_GCM SHA384))
+  | ( 0x00z, 0xA4z ) -> Correct(CipherSuite Kex_DH (Some DSA)  (AEAD AES_128_GCM SHA256))
+  | ( 0x00z, 0xA5z ) -> Correct(CipherSuite Kex_DH (Some DSA)  (AEAD AES_256_GCM SHA384))
 
-    | ( 0x00z, 0xA6z ) -> Correct(CipherSuite Kex_DHE None (AEAD AES_128_GCM SHA256))
-    | ( 0x00z, 0xA7z ) -> Correct(CipherSuite Kex_DHE None (AEAD AES_256_GCM SHA384))
+  | ( 0x00z, 0xA6z ) -> Correct(CipherSuite Kex_DHE None (AEAD AES_128_GCM SHA256))
+  | ( 0x00z, 0xA7z ) -> Correct(CipherSuite Kex_DHE None (AEAD AES_256_GCM SHA384))
 
-    | ( 0x00z, 0xFFz ) -> Correct(SCSV (TLS_EMPTY_RENEGOTIATION_INFO_SCSV))
+  | ( 0x00z, 0xFFz ) -> Correct(SCSV (TLS_EMPTY_RENEGOTIATION_INFO_SCSV))
 
-    | _ -> Error(AD_decode_error, perror __SOURCE_FILE__ __LINE__ "Parsed unknown cipher")
+  | _ -> Error(AD_decode_error, perror __SOURCE_FILE__ __LINE__ "Parsed unknown cipher")
 
-val parseCipherSuite : pinverse_t cipherSuiteBytes
+val parseCipherSuite: pinverse_t cipherSuiteBytes
 let parseCipherSuite b =
   match parseCipherSuiteAux b with
   | Correct c -> Correct c
   | Error z -> Error z
 
-
 #set-options "--max_ifuel 6 --initial_ifuel 6 --max_fuel 1 --initial_fuel 1"
 val inverse_cipherSuite: x:cipherSuite -> Lemma
-   (requires (True))
-   (ensures (let y = cipherSuiteBytesOpt x in
-		(is_Some y ==> parseCipherSuiteAux (Some.v y) = Correct x)))
-   [SMTPat (parseCipherSuiteAux (Some.v (cipherSuiteBytesOpt x)))]
+  (requires (True))
+  (ensures (let y = cipherSuiteBytesOpt x in
+	(is_Some y ==> parseCipherSuiteAux (Some.v y) = Correct x)))
+  [SMTPat (parseCipherSuiteAux (Some.v (cipherSuiteBytesOpt x)))]
 let inverse_cipherSuite x = ()
 
 val pinverse_cipherSuite : x:lbytes 2 -> Lemma
@@ -498,78 +489,101 @@ let pinverse_cipherSuite x = ()
 #reset-options
 #set-options "--max_ifuel 1 --initial_ifuel 1 --max_fuel 1 --initial_fuel 1"
 
-
 (* Called by the server handshake; *)
 (* ciphersuites that we do not understand are parsed, but ignored *)
 val parseCipherSuites: b:bytes -> Tot (result known_cipher_suites) (decreases (length b))
 let rec parseCipherSuites b : result known_cipher_suites =
-     if length b > 1 then
-       let (b0,b1) = split b 2 in
-       match parseCipherSuites b1 with
-         | Correct(css) ->
-           (match parseCipherSuite b0 with
-             | Error(z) ->    Correct (css)      (* ignore this cs *)
-             | Correct(cs) -> Correct(cs::css))
-         | Error(z) -> Error(z)
-     else if length b = 0 then Correct ([])
-     else Error(AD_decode_error, perror __SOURCE_FILE__ __LINE__ "Odd cs bytes number")
+  if length b > 1 then
+    let (b0,b1) = split b 2 in
+    match parseCipherSuites b1 with
+      | Correct(css) ->
+	(match parseCipherSuite b0 with
+	 | Error z ->	Correct css       (* ignore this cs *)
+	 | Correct cs -> Correct (cs::css))
+      | Error z -> Error z
+  else
+  if length b = 0 then Correct []
+  else Error(AD_decode_error, perror __SOURCE_FILE__ __LINE__ "Odd cs bytes number")
 
 val cipherSuitesBytes: css:known_cipher_suites -> Tot (lbytes (op_Multiply 2 (List.Tot.length css)))
 let rec cipherSuitesBytes css =
-   match css with
-     | [] -> empty_bytes
-     | cs::css -> (cipherSuiteBytes cs) @| (cipherSuitesBytes css)
+  match css with
+  | [] -> empty_bytes
+  | cs::css -> (cipherSuiteBytes cs) @| (cipherSuitesBytes css)
+  
+val inverse_cipherSuites: x:known_cipher_suites -> Lemma
+  (requires (True))
+  (ensures (parseCipherSuites (cipherSuitesBytes x) = Correct x))
+  [SMTPat (parseCipherSuites (cipherSuitesBytes x))]
+let rec inverse_cipherSuites x =
+  match x with
+  | [] -> ()
+  | cs::css -> 
+    let b = (cipherSuiteBytes cs) @| (cipherSuitesBytes css) in
+    let (b0,b1) = split b 2 in
+    lemma_split b 2;
+    lemma_append_inj b0 b1 (cipherSuiteBytes cs) (cipherSuitesBytes css);  
+    inverse_cipherSuites css
+
+(* 
+  REMARK: cipherSuitesBytes is not a partial inverse of parseCipherSuites,
+  because parseCipherSuites drops unknown ciphersuites.
+  Alternatively, we could add an UNKNOWN of (lbyte 2) constructor in cipherSuite
+  to make this hold.
+*)
 
 let isAnonCipherSuite cs =
-    match cs with
-    | CipherSuite Kex_DHE None _    -> true
-    | _ -> false
+  match cs with
+  | CipherSuite Kex_DHE None _ -> true
+  | _ -> false
 
 let isDHECipherSuite cs =
-    match cs with
-    | CipherSuite Kex_DHE (Some DSA) _      -> true
-    | CipherSuite Kex_DHE (Some RSASIG) _   -> true
-    | CipherSuite Kex_ECDHE (Some ECDSA) _  -> true
-    | CipherSuite Kex_ECDHE (Some RSASIG) _ -> true
-    | _ -> false
+  match cs with
+  | CipherSuite Kex_DHE (Some DSA) _      -> true
+  | CipherSuite Kex_DHE (Some RSASIG) _   -> true
+  | CipherSuite Kex_ECDHE (Some ECDSA) _  -> true
+  | CipherSuite Kex_ECDHE (Some RSASIG) _ -> true
+  | _ -> false
 
 let isECDHECipherSuite cs =
-    match cs with
-    | CipherSuite Kex_ECDHE (Some ECDSA) _  -> true
-    | CipherSuite Kex_ECDHE (Some RSASIG) _ -> true
-    | _ -> false
+  match cs with
+  | CipherSuite Kex_ECDHE (Some ECDSA) _  -> true
+  | CipherSuite Kex_ECDHE (Some RSASIG) _ -> true
+  | _ -> false
 
 let isDHCipherSuite cs =
-    match cs with
-    | CipherSuite Kex_DH (Some DSA) _    -> true
-    | CipherSuite Kex_DH (Some RSASIG) _ -> true
-    | _ -> false
+  match cs with
+  | CipherSuite Kex_DH (Some DSA) _    -> true
+  | CipherSuite Kex_DH (Some RSASIG) _ -> true
+  | _ -> false
 
 let isRSACipherSuite cs =
-    match cs with
-    | CipherSuite Kex_RSA None _ -> true
-    | _ -> false
+  match cs with
+  | CipherSuite Kex_RSA None _ -> true
+  | _ -> false
 
 let isOnlyMACCipherSuite cs =
-    match cs with
-    | CipherSuite _ _ (MACOnly _) -> true
-    | _ -> false
+  match cs with
+  | CipherSuite _ _ (MACOnly _) -> true
+  | _ -> false
 
 let sigAlg_of_ciphersuite cs =
-    match cs with
-    | CipherSuite Kex_RSA None _
-    | CipherSuite Kex_ECDHE (Some RSASIG) _
-    | CipherSuite Kex_DHE (Some RSASIG) _
-    | CipherSuite Kex_DH (Some RSASIG) _   -> RSASIG
-    | CipherSuite Kex_DHE (Some DSA) _
-    | CipherSuite Kex_DH (Some DSA) _      -> DSA
-    | CipherSuite Kex_ECDHE (Some ECDSA) _ -> ECDSA
-    | _ -> unexpected "[sigAlg_of_ciphersuite] invoked on a wrong ciphersuite"
+  match cs with
+  | CipherSuite Kex_RSA None _
+  | CipherSuite Kex_ECDHE (Some RSASIG) _
+  | CipherSuite Kex_DHE (Some RSASIG) _
+  | CipherSuite Kex_DH (Some RSASIG) _   -> RSASIG
+  | CipherSuite Kex_DHE (Some DSA) _
+  | CipherSuite Kex_DH (Some DSA) _      -> DSA
+  | CipherSuite Kex_ECDHE (Some ECDSA) _ -> ECDSA
+  | _ -> unexpected "[sigAlg_of_ciphersuite] invoked on a wrong ciphersuite"
+
 
 type prflabel = bytes
-let extract_label = utf8 "master secret"
+
+let extract_label          = utf8 "master secret"
 let extended_extract_label = utf8 "extended master secret"
-let kdf_label     = utf8 "key expansion"
+let kdf_label              = utf8 "key expansion"
 
 type prePrfAlg =
   | PRF_SSL3_nested         // MD5(SHA1(...)) for extraction and keygen
@@ -588,10 +602,10 @@ let verifyDataLen_of_ciphersuite (cs:cipherSuite) = 12
 (* Only to be invoked with TLS 1.2 (hardcoded in previous versions *)
 val prfMacAlg_of_ciphersuite_aux: cipherSuite -> Tot (option macAlg)
 let prfMacAlg_of_ciphersuite_aux = function
-    | CipherSuite  _ _  (MtE  _ _ )   -> Some (HMAC SHA256)
-    | CipherSuite  _ _  (AEAD _ hAlg) -> Some (HMAC hAlg)
-    | CipherSuite  _ _  (MACOnly _)  -> Some (HMAC SHA256) //MK was (MACOnly hAlg) should it also be be (HMAC hAlg)?
-    | _                                -> None
+  | CipherSuite  _ _  (MtE  _ _ )   -> Some (HMAC SHA256)
+  | CipherSuite  _ _  (AEAD _ hAlg) -> Some (HMAC hAlg)
+  | CipherSuite  _ _  (MACOnly _)   -> Some (HMAC SHA256) //MK was (MACOnly hAlg) should it also be be (HMAC hAlg)?
+  | _                               -> None
 
 let pvcs (pv:protocolVersion) (cs:cipherSuite) =
   match pv with
@@ -619,238 +633,248 @@ let verifyDataHashAlg_of_ciphersuite : require_some verifyDataHashAlg_of_ciphers
 
 val sessionHashAlg: pv:protocolVersion -> cs:cipherSuite{pvcs pv cs} -> Tot hashAlg
 let sessionHashAlg pv cs =
-    match pv with
-    | SSL_3p0 | TLS_1p0 | TLS_1p1 -> MD5SHA1
-    | TLS_1p2 | TLS_1p3           -> Hash (verifyDataHashAlg_of_ciphersuite cs)
+  match pv with
+  | SSL_3p0 | TLS_1p0 | TLS_1p1 -> MD5SHA1
+  | TLS_1p2 | TLS_1p3           -> Hash (verifyDataHashAlg_of_ciphersuite cs)
 // TODO recheck this is the right hash for HKDF
+// SZ: Right. The TLS 1.3 draft says "Where HMAC [RFC2104] uses
+// the Hash algorithm for the handshake"
 
 val get_aeAlg: cs:cipherSuite{ is_CipherSuite cs } -> Tot aeAlg
 let get_aeAlg cs =
-    match cs with
-    | CipherSuite _ _ ae -> ae
+  match cs with
+  | CipherSuite _ _ ae -> ae
 
-let null_aeAlg  = MACOnly MD5
+let null_aeAlg = MACOnly MD5
 
 val encAlg_of_aeAlg: (pv:protocolVersion) -> (a:aeAlg { is_MtE a }) -> Tot (encAlg * ivMode)
 let encAlg_of_aeAlg  pv ae =
-    match pv,ae with
-    | SSL_3p0, MtE (Block e) m -> (Block e),Stale
-    | TLS_1p0, MtE (Block e) m -> (Block e),Stale
-    | _, MtE e m -> e,Fresh
+  match pv,ae with
+  | SSL_3p0, MtE (Block e) m -> (Block e),Stale
+  | TLS_1p0, MtE (Block e) m -> (Block e),Stale
+  | _, MtE e m -> e,Fresh
 
 val macAlg_of_aeAlg: (pv:protocolVersion) -> (a:aeAlg { pv <> TLS_1p3 /\ ~(is_AEAD a) }) -> Tot macAlg
 let macAlg_of_aeAlg pv ae =
-    match pv,ae with
-//  | SSL_3p0,MACOnly alg -> SSLKHASH alg (* dropped pattern on the left to simplify refinements *)
-    | _      ,MACOnly alg -> SSLKHASH alg
-    | SSL_3p0,MtE _ alg   -> SSLKHASH alg
-    | _      ,MtE _ alg   -> HMAC alg
+  match pv,ae with
+  | SSL_3p0,MACOnly alg -> SSLKHASH alg (* dropped pattern on the left to simplify refinements *)
+  | _      ,MACOnly alg -> SSLKHASH alg
+  | SSL_3p0,MtE _ alg   -> SSLKHASH alg
+  | _      ,MtE _ alg   -> HMAC alg
 
 type cipherSuiteName =
-    | TLS_NULL_WITH_NULL_NULL
+  | TLS_NULL_WITH_NULL_NULL
 
-    | TLS_RSA_WITH_NULL_MD5
-    | TLS_RSA_WITH_NULL_SHA
-    | TLS_RSA_WITH_NULL_SHA256
-    | TLS_RSA_WITH_RC4_128_MD5
-    | TLS_RSA_WITH_RC4_128_SHA
-    | TLS_RSA_WITH_3DES_EDE_CBC_SHA
-    | TLS_RSA_WITH_AES_128_CBC_SHA
-    | TLS_RSA_WITH_AES_256_CBC_SHA
-    | TLS_RSA_WITH_AES_128_CBC_SHA256
-    | TLS_RSA_WITH_AES_256_CBC_SHA256
+  | TLS_RSA_WITH_NULL_MD5
+  | TLS_RSA_WITH_NULL_SHA
+  | TLS_RSA_WITH_NULL_SHA256
+  | TLS_RSA_WITH_RC4_128_MD5
+  | TLS_RSA_WITH_RC4_128_SHA
+  | TLS_RSA_WITH_3DES_EDE_CBC_SHA
+  | TLS_RSA_WITH_AES_128_CBC_SHA
+  | TLS_RSA_WITH_AES_256_CBC_SHA
+  | TLS_RSA_WITH_AES_128_CBC_SHA256
+  | TLS_RSA_WITH_AES_256_CBC_SHA256
 
-    | TLS_DHE_DSS_WITH_3DES_EDE_CBC_SHA
-    | TLS_DHE_RSA_WITH_3DES_EDE_CBC_SHA
-    | TLS_DHE_DSS_WITH_AES_128_CBC_SHA
-    | TLS_DHE_RSA_WITH_AES_128_CBC_SHA
-    | TLS_DHE_DSS_WITH_AES_256_CBC_SHA
-    | TLS_DHE_RSA_WITH_AES_256_CBC_SHA
-    | TLS_DHE_DSS_WITH_AES_128_CBC_SHA256
-    | TLS_DHE_RSA_WITH_AES_128_CBC_SHA256
-    | TLS_DHE_DSS_WITH_AES_256_CBC_SHA256
-    | TLS_DHE_RSA_WITH_AES_256_CBC_SHA256
+  | TLS_DHE_DSS_WITH_3DES_EDE_CBC_SHA
+  | TLS_DHE_RSA_WITH_3DES_EDE_CBC_SHA
+  | TLS_DHE_DSS_WITH_AES_128_CBC_SHA
+  | TLS_DHE_RSA_WITH_AES_128_CBC_SHA
+  | TLS_DHE_DSS_WITH_AES_256_CBC_SHA
+  | TLS_DHE_RSA_WITH_AES_256_CBC_SHA
+  | TLS_DHE_DSS_WITH_AES_128_CBC_SHA256
+  | TLS_DHE_RSA_WITH_AES_128_CBC_SHA256
+  | TLS_DHE_DSS_WITH_AES_256_CBC_SHA256
+  | TLS_DHE_RSA_WITH_AES_256_CBC_SHA256
 
-    | TLS_ECDHE_RSA_WITH_RC4_128_SHA
-    | TLS_ECDHE_RSA_WITH_3DES_EDE_CBC_SHA
-    | TLS_ECDHE_RSA_WITH_AES_128_CBC_SHA
-    | TLS_ECDHE_RSA_WITH_AES_128_CBC_SHA256
-    | TLS_ECDHE_RSA_WITH_AES_256_CBC_SHA
-    | TLS_ECDHE_RSA_WITH_AES_256_CBC_SHA384
+  | TLS_ECDHE_RSA_WITH_RC4_128_SHA
+  | TLS_ECDHE_RSA_WITH_3DES_EDE_CBC_SHA
+  | TLS_ECDHE_RSA_WITH_AES_128_CBC_SHA
+  | TLS_ECDHE_RSA_WITH_AES_128_CBC_SHA256
+  | TLS_ECDHE_RSA_WITH_AES_256_CBC_SHA
+  | TLS_ECDHE_RSA_WITH_AES_256_CBC_SHA384
 
-    | TLS_ECDHE_RSA_WITH_AES_128_GCM_SHA256
-    | TLS_ECDHE_RSA_WITH_AES_256_GCM_SHA384
+  | TLS_ECDHE_RSA_WITH_AES_128_GCM_SHA256
+  | TLS_ECDHE_RSA_WITH_AES_256_GCM_SHA384
 
-    | TLS_DH_anon_WITH_RC4_128_MD5
-    | TLS_DH_anon_WITH_3DES_EDE_CBC_SHA
-    | TLS_DH_anon_WITH_AES_128_CBC_SHA
-    | TLS_DH_anon_WITH_AES_256_CBC_SHA
-    | TLS_DH_anon_WITH_AES_128_CBC_SHA256
-    | TLS_DH_anon_WITH_AES_256_CBC_SHA256
+  | TLS_DH_anon_WITH_RC4_128_MD5
+  | TLS_DH_anon_WITH_3DES_EDE_CBC_SHA
+  | TLS_DH_anon_WITH_AES_128_CBC_SHA
+  | TLS_DH_anon_WITH_AES_256_CBC_SHA
+  | TLS_DH_anon_WITH_AES_128_CBC_SHA256
+  | TLS_DH_anon_WITH_AES_256_CBC_SHA256
 
-    | TLS_RSA_WITH_AES_128_GCM_SHA256
-    | TLS_RSA_WITH_AES_256_GCM_SHA384
-    | TLS_DHE_RSA_WITH_AES_128_GCM_SHA256
-    | TLS_DHE_RSA_WITH_AES_256_GCM_SHA384
-    | TLS_DH_RSA_WITH_AES_128_GCM_SHA256
-    | TLS_DH_RSA_WITH_AES_256_GCM_SHA384
-    | TLS_DHE_DSS_WITH_AES_128_GCM_SHA256
-    | TLS_DHE_DSS_WITH_AES_256_GCM_SHA384
-    | TLS_DH_DSS_WITH_AES_128_GCM_SHA256
-    | TLS_DH_DSS_WITH_AES_256_GCM_SHA384
-    | TLS_DH_anon_WITH_AES_128_GCM_SHA256
-    | TLS_DH_anon_WITH_AES_256_GCM_SHA384
+  | TLS_RSA_WITH_AES_128_GCM_SHA256
+  | TLS_RSA_WITH_AES_256_GCM_SHA384
+  | TLS_DHE_RSA_WITH_AES_128_GCM_SHA256
+  | TLS_DHE_RSA_WITH_AES_256_GCM_SHA384
+  | TLS_DH_RSA_WITH_AES_128_GCM_SHA256
+  | TLS_DH_RSA_WITH_AES_256_GCM_SHA384
+  | TLS_DHE_DSS_WITH_AES_128_GCM_SHA256
+  | TLS_DHE_DSS_WITH_AES_256_GCM_SHA384
+  | TLS_DH_DSS_WITH_AES_128_GCM_SHA256
+  | TLS_DH_DSS_WITH_AES_256_GCM_SHA384
+  | TLS_DH_anon_WITH_AES_128_GCM_SHA256
+  | TLS_DH_anon_WITH_AES_256_GCM_SHA384
 
 type cipherSuiteNames = list cipherSuiteName
 
 val cipherSuite_of_name: cipherSuiteName -> Tot known_cipher_suite
 let cipherSuite_of_name = function
-    | TLS_NULL_WITH_NULL_NULL                -> NullCipherSuite
+  | TLS_NULL_WITH_NULL_NULL                -> NullCipherSuite
 
-    | TLS_RSA_WITH_NULL_MD5                  -> CipherSuite Kex_RSA None (MACOnly MD5)
-    | TLS_RSA_WITH_NULL_SHA                  -> CipherSuite Kex_RSA None (MACOnly SHA1)
-    | TLS_RSA_WITH_NULL_SHA256               -> CipherSuite Kex_RSA None (MACOnly SHA256)
-    | TLS_RSA_WITH_RC4_128_MD5               -> CipherSuite Kex_RSA None (MtE (Stream RC4_128) MD5)
-    | TLS_RSA_WITH_RC4_128_SHA               -> CipherSuite Kex_RSA None (MtE (Stream RC4_128) SHA1)
-    | TLS_RSA_WITH_3DES_EDE_CBC_SHA          -> CipherSuite Kex_RSA None (MtE (Block TDES_EDE_CBC) SHA1)
-    | TLS_RSA_WITH_AES_128_CBC_SHA           -> CipherSuite Kex_RSA None (MtE (Block AES_128_CBC) SHA1)
-    | TLS_RSA_WITH_AES_256_CBC_SHA           -> CipherSuite Kex_RSA None (MtE (Block AES_256_CBC) SHA1)
-    | TLS_RSA_WITH_AES_128_CBC_SHA256        -> CipherSuite Kex_RSA None (MtE (Block AES_128_CBC) SHA256)
-    | TLS_RSA_WITH_AES_256_CBC_SHA256        -> CipherSuite Kex_RSA None (MtE (Block AES_256_CBC) SHA256)
+  | TLS_RSA_WITH_NULL_MD5                  -> CipherSuite Kex_RSA None (MACOnly MD5)
+  | TLS_RSA_WITH_NULL_SHA                  -> CipherSuite Kex_RSA None (MACOnly SHA1)
+  | TLS_RSA_WITH_NULL_SHA256               -> CipherSuite Kex_RSA None (MACOnly SHA256)
+  | TLS_RSA_WITH_RC4_128_MD5               -> CipherSuite Kex_RSA None (MtE (Stream RC4_128) MD5)
+  | TLS_RSA_WITH_RC4_128_SHA               -> CipherSuite Kex_RSA None (MtE (Stream RC4_128) SHA1)
+  | TLS_RSA_WITH_3DES_EDE_CBC_SHA          -> CipherSuite Kex_RSA None (MtE (Block TDES_EDE_CBC) SHA1)
+  | TLS_RSA_WITH_AES_128_CBC_SHA           -> CipherSuite Kex_RSA None (MtE (Block AES_128_CBC) SHA1)
+  | TLS_RSA_WITH_AES_256_CBC_SHA           -> CipherSuite Kex_RSA None (MtE (Block AES_256_CBC) SHA1)
+  | TLS_RSA_WITH_AES_128_CBC_SHA256        -> CipherSuite Kex_RSA None (MtE (Block AES_128_CBC) SHA256)
+  | TLS_RSA_WITH_AES_256_CBC_SHA256        -> CipherSuite Kex_RSA None (MtE (Block AES_256_CBC) SHA256)
 
-    | TLS_DHE_DSS_WITH_3DES_EDE_CBC_SHA      -> CipherSuite Kex_DHE (Some DSA) (MtE (Block TDES_EDE_CBC) SHA1)
-    | TLS_DHE_RSA_WITH_3DES_EDE_CBC_SHA      -> CipherSuite Kex_DHE (Some RSASIG) (MtE (Block TDES_EDE_CBC) SHA1)
-    | TLS_DHE_DSS_WITH_AES_128_CBC_SHA       -> CipherSuite Kex_DHE (Some DSA) (MtE (Block AES_128_CBC) SHA1)
-    | TLS_DHE_RSA_WITH_AES_128_CBC_SHA       -> CipherSuite Kex_DHE (Some RSASIG) (MtE (Block AES_128_CBC) SHA1)
-    | TLS_DHE_DSS_WITH_AES_256_CBC_SHA       -> CipherSuite Kex_DHE (Some DSA) (MtE (Block AES_256_CBC) SHA1)
-    | TLS_DHE_RSA_WITH_AES_256_CBC_SHA       -> CipherSuite Kex_DHE (Some RSASIG) (MtE (Block AES_256_CBC) SHA1)
-    | TLS_DHE_DSS_WITH_AES_128_CBC_SHA256    -> CipherSuite Kex_DHE (Some DSA) (MtE (Block AES_128_CBC) SHA256)
-    | TLS_DHE_RSA_WITH_AES_128_CBC_SHA256    -> CipherSuite Kex_DHE (Some RSASIG) (MtE (Block AES_128_CBC) SHA256)
-    | TLS_DHE_DSS_WITH_AES_256_CBC_SHA256    -> CipherSuite Kex_DHE (Some DSA) (MtE (Block AES_256_CBC) SHA256)
-    | TLS_DHE_RSA_WITH_AES_256_CBC_SHA256    -> CipherSuite Kex_DHE (Some RSASIG) (MtE (Block AES_256_CBC) SHA256)
+  | TLS_DHE_DSS_WITH_3DES_EDE_CBC_SHA      -> CipherSuite Kex_DHE (Some DSA) (MtE (Block TDES_EDE_CBC) SHA1)
+  | TLS_DHE_RSA_WITH_3DES_EDE_CBC_SHA      -> CipherSuite Kex_DHE (Some RSASIG) (MtE (Block TDES_EDE_CBC) SHA1)
+  | TLS_DHE_DSS_WITH_AES_128_CBC_SHA       -> CipherSuite Kex_DHE (Some DSA) (MtE (Block AES_128_CBC) SHA1)
+  | TLS_DHE_RSA_WITH_AES_128_CBC_SHA       -> CipherSuite Kex_DHE (Some RSASIG) (MtE (Block AES_128_CBC) SHA1)
+  | TLS_DHE_DSS_WITH_AES_256_CBC_SHA       -> CipherSuite Kex_DHE (Some DSA) (MtE (Block AES_256_CBC) SHA1)
+  | TLS_DHE_RSA_WITH_AES_256_CBC_SHA       -> CipherSuite Kex_DHE (Some RSASIG) (MtE (Block AES_256_CBC) SHA1)
+  | TLS_DHE_DSS_WITH_AES_128_CBC_SHA256    -> CipherSuite Kex_DHE (Some DSA) (MtE (Block AES_128_CBC) SHA256)
+  | TLS_DHE_RSA_WITH_AES_128_CBC_SHA256    -> CipherSuite Kex_DHE (Some RSASIG) (MtE (Block AES_128_CBC) SHA256)
+  | TLS_DHE_DSS_WITH_AES_256_CBC_SHA256    -> CipherSuite Kex_DHE (Some DSA) (MtE (Block AES_256_CBC) SHA256)
+  | TLS_DHE_RSA_WITH_AES_256_CBC_SHA256    -> CipherSuite Kex_DHE (Some RSASIG) (MtE (Block AES_256_CBC) SHA256)
 
-    | TLS_ECDHE_RSA_WITH_RC4_128_SHA         -> CipherSuite Kex_ECDHE (Some RSASIG) (MtE (Stream RC4_128) SHA1)
-    | TLS_ECDHE_RSA_WITH_3DES_EDE_CBC_SHA    -> CipherSuite Kex_ECDHE (Some RSASIG) (MtE (Block TDES_EDE_CBC) SHA1)
-    | TLS_ECDHE_RSA_WITH_AES_128_CBC_SHA     -> CipherSuite Kex_ECDHE (Some RSASIG) (MtE (Block AES_128_CBC) SHA1)
-    | TLS_ECDHE_RSA_WITH_AES_128_CBC_SHA256  -> CipherSuite Kex_ECDHE (Some RSASIG) (MtE (Block AES_128_CBC) SHA256)
-    | TLS_ECDHE_RSA_WITH_AES_256_CBC_SHA     -> CipherSuite Kex_ECDHE (Some RSASIG) (MtE (Block AES_256_CBC) SHA1)
-    | TLS_ECDHE_RSA_WITH_AES_256_CBC_SHA384  -> CipherSuite Kex_ECDHE (Some RSASIG) (MtE (Block AES_256_CBC) SHA384)
+  | TLS_ECDHE_RSA_WITH_RC4_128_SHA         -> CipherSuite Kex_ECDHE (Some RSASIG) (MtE (Stream RC4_128) SHA1)
+  | TLS_ECDHE_RSA_WITH_3DES_EDE_CBC_SHA    -> CipherSuite Kex_ECDHE (Some RSASIG) (MtE (Block TDES_EDE_CBC) SHA1)
+  | TLS_ECDHE_RSA_WITH_AES_128_CBC_SHA     -> CipherSuite Kex_ECDHE (Some RSASIG) (MtE (Block AES_128_CBC) SHA1)
+  | TLS_ECDHE_RSA_WITH_AES_128_CBC_SHA256  -> CipherSuite Kex_ECDHE (Some RSASIG) (MtE (Block AES_128_CBC) SHA256)
+  | TLS_ECDHE_RSA_WITH_AES_256_CBC_SHA     -> CipherSuite Kex_ECDHE (Some RSASIG) (MtE (Block AES_256_CBC) SHA1)
+  | TLS_ECDHE_RSA_WITH_AES_256_CBC_SHA384  -> CipherSuite Kex_ECDHE (Some RSASIG) (MtE (Block AES_256_CBC) SHA384)
 
-    | TLS_ECDHE_RSA_WITH_AES_128_GCM_SHA256  -> CipherSuite Kex_ECDHE (Some RSASIG) (AEAD AES_128_GCM SHA256)
-    | TLS_ECDHE_RSA_WITH_AES_256_GCM_SHA384  -> CipherSuite Kex_ECDHE (Some RSASIG) (AEAD AES_256_GCM SHA384)
+  | TLS_ECDHE_RSA_WITH_AES_128_GCM_SHA256  -> CipherSuite Kex_ECDHE (Some RSASIG) (AEAD AES_128_GCM SHA256)
+  | TLS_ECDHE_RSA_WITH_AES_256_GCM_SHA384  -> CipherSuite Kex_ECDHE (Some RSASIG) (AEAD AES_256_GCM SHA384)
 
-    | TLS_DH_anon_WITH_RC4_128_MD5           -> CipherSuite Kex_DHE None (MtE (Stream RC4_128) MD5)
-    | TLS_DH_anon_WITH_3DES_EDE_CBC_SHA      -> CipherSuite Kex_DHE None (MtE (Block TDES_EDE_CBC) SHA1)
-    | TLS_DH_anon_WITH_AES_128_CBC_SHA       -> CipherSuite Kex_DHE None (MtE (Block AES_128_CBC) SHA1)
-    | TLS_DH_anon_WITH_AES_256_CBC_SHA       -> CipherSuite Kex_DHE None (MtE (Block AES_256_CBC) SHA1)
-    | TLS_DH_anon_WITH_AES_128_CBC_SHA256    -> CipherSuite Kex_DHE None (MtE (Block AES_128_CBC) SHA256)
-    | TLS_DH_anon_WITH_AES_256_CBC_SHA256    -> CipherSuite Kex_DHE None (MtE (Block AES_256_CBC) SHA256)
+  | TLS_DH_anon_WITH_RC4_128_MD5           -> CipherSuite Kex_DHE None (MtE (Stream RC4_128) MD5)
+  | TLS_DH_anon_WITH_3DES_EDE_CBC_SHA      -> CipherSuite Kex_DHE None (MtE (Block TDES_EDE_CBC) SHA1)
+  | TLS_DH_anon_WITH_AES_128_CBC_SHA       -> CipherSuite Kex_DHE None (MtE (Block AES_128_CBC) SHA1)
+  | TLS_DH_anon_WITH_AES_256_CBC_SHA       -> CipherSuite Kex_DHE None (MtE (Block AES_256_CBC) SHA1)
+  | TLS_DH_anon_WITH_AES_128_CBC_SHA256    -> CipherSuite Kex_DHE None (MtE (Block AES_128_CBC) SHA256)
+  | TLS_DH_anon_WITH_AES_256_CBC_SHA256    -> CipherSuite Kex_DHE None (MtE (Block AES_256_CBC) SHA256)
 
-    | TLS_RSA_WITH_AES_128_GCM_SHA256        -> CipherSuite Kex_RSA None     (AEAD AES_128_GCM SHA256)
-    | TLS_RSA_WITH_AES_256_GCM_SHA384        -> CipherSuite Kex_RSA None     (AEAD AES_256_GCM SHA384)
-    | TLS_DHE_RSA_WITH_AES_128_GCM_SHA256    -> CipherSuite Kex_DHE (Some RSASIG) (AEAD AES_128_GCM SHA256)
-    | TLS_DHE_RSA_WITH_AES_256_GCM_SHA384    -> CipherSuite Kex_DHE (Some RSASIG) (AEAD AES_256_GCM SHA384)
-    | TLS_DH_RSA_WITH_AES_128_GCM_SHA256     -> CipherSuite Kex_DH (Some RSASIG)  (AEAD AES_128_GCM SHA256)
-    | TLS_DH_RSA_WITH_AES_256_GCM_SHA384     -> CipherSuite Kex_DH (Some RSASIG)  (AEAD AES_256_GCM SHA384)
-    | TLS_DHE_DSS_WITH_AES_128_GCM_SHA256    -> CipherSuite Kex_DHE (Some DSA) (AEAD AES_128_GCM SHA256)
-    | TLS_DHE_DSS_WITH_AES_256_GCM_SHA384    -> CipherSuite Kex_DHE (Some DSA) (AEAD AES_256_GCM SHA384)
-    | TLS_DH_DSS_WITH_AES_128_GCM_SHA256     -> CipherSuite Kex_DH (Some DSA)  (AEAD AES_128_GCM SHA256)
-    | TLS_DH_DSS_WITH_AES_256_GCM_SHA384     -> CipherSuite Kex_DH (Some DSA)  (AEAD AES_256_GCM SHA384)
-    | TLS_DH_anon_WITH_AES_128_GCM_SHA256    -> CipherSuite Kex_DHE None (AEAD AES_128_GCM SHA256)
-    | TLS_DH_anon_WITH_AES_256_GCM_SHA384    -> CipherSuite Kex_DHE None (AEAD AES_256_GCM SHA384)
+  | TLS_RSA_WITH_AES_128_GCM_SHA256        -> CipherSuite Kex_RSA None          (AEAD AES_128_GCM SHA256)
+  | TLS_RSA_WITH_AES_256_GCM_SHA384        -> CipherSuite Kex_RSA None          (AEAD AES_256_GCM SHA384)
+  | TLS_DHE_RSA_WITH_AES_128_GCM_SHA256    -> CipherSuite Kex_DHE (Some RSASIG) (AEAD AES_128_GCM SHA256)
+  | TLS_DHE_RSA_WITH_AES_256_GCM_SHA384    -> CipherSuite Kex_DHE (Some RSASIG) (AEAD AES_256_GCM SHA384)
+  | TLS_DH_RSA_WITH_AES_128_GCM_SHA256     -> CipherSuite Kex_DH  (Some RSASIG) (AEAD AES_128_GCM SHA256)
+  | TLS_DH_RSA_WITH_AES_256_GCM_SHA384     -> CipherSuite Kex_DH  (Some RSASIG) (AEAD AES_256_GCM SHA384)
+  | TLS_DHE_DSS_WITH_AES_128_GCM_SHA256    -> CipherSuite Kex_DHE (Some DSA)    (AEAD AES_128_GCM SHA256)
+  | TLS_DHE_DSS_WITH_AES_256_GCM_SHA384    -> CipherSuite Kex_DHE (Some DSA)    (AEAD AES_256_GCM SHA384)
+  | TLS_DH_DSS_WITH_AES_128_GCM_SHA256     -> CipherSuite Kex_DH  (Some DSA)    (AEAD AES_128_GCM SHA256)
+  | TLS_DH_DSS_WITH_AES_256_GCM_SHA384     -> CipherSuite Kex_DH  (Some DSA)    (AEAD AES_256_GCM SHA384)
+  | TLS_DH_anon_WITH_AES_128_GCM_SHA256    -> CipherSuite Kex_DHE None          (AEAD AES_128_GCM SHA256)
+  | TLS_DH_anon_WITH_AES_256_GCM_SHA384    -> CipherSuite Kex_DHE None          (AEAD AES_256_GCM SHA384)
 
-val cipherSuites_of_nameList: l1:list cipherSuiteName -> l2:known_cipher_suites{List.Tot.length l2 = List.Tot.length l1}
+val cipherSuites_of_nameList: l1:list cipherSuiteName 
+  -> l2:known_cipher_suites{List.Tot.length l2 = List.Tot.length l1}
 let cipherSuites_of_nameList nameList = List.Tot.map cipherSuite_of_name nameList
 
 let name_of_cipherSuite cs =
-    match cs with
-    | NullCipherSuite                                  ->  Correct TLS_NULL_WITH_NULL_NULL
+  match cs with
+  | NullCipherSuite                                                      -> Correct TLS_NULL_WITH_NULL_NULL
 
-    | CipherSuite Kex_RSA None (MACOnly MD5)                       ->  Correct TLS_RSA_WITH_NULL_MD5
-    | CipherSuite Kex_RSA None (MACOnly SHA1)                       ->  Correct TLS_RSA_WITH_NULL_SHA
-    | CipherSuite Kex_RSA None (MACOnly SHA256)                    ->  Correct TLS_RSA_WITH_NULL_SHA256
-    | CipherSuite Kex_RSA None (MtE (Stream RC4_128) MD5)             ->  Correct TLS_RSA_WITH_RC4_128_MD5
-    | CipherSuite Kex_RSA None (MtE (Stream RC4_128) SHA1)             ->  Correct TLS_RSA_WITH_RC4_128_SHA
-    | CipherSuite Kex_RSA None (MtE (Block TDES_EDE_CBC) SHA1)        ->  Correct TLS_RSA_WITH_3DES_EDE_CBC_SHA
-    | CipherSuite Kex_RSA None (MtE (Block AES_128_CBC) SHA1)         ->  Correct TLS_RSA_WITH_AES_128_CBC_SHA
-    | CipherSuite Kex_RSA None (MtE (Block AES_256_CBC) SHA1)         ->  Correct TLS_RSA_WITH_AES_256_CBC_SHA
-    | CipherSuite Kex_RSA None (MtE (Block AES_128_CBC) SHA256)      ->  Correct TLS_RSA_WITH_AES_128_CBC_SHA256
-    | CipherSuite Kex_RSA None (MtE (Block AES_256_CBC) SHA256)      ->  Correct TLS_RSA_WITH_AES_256_CBC_SHA256
+  | CipherSuite Kex_RSA None (MACOnly MD5)                               -> Correct TLS_RSA_WITH_NULL_MD5
+  | CipherSuite Kex_RSA None (MACOnly SHA1)                              -> Correct TLS_RSA_WITH_NULL_SHA
+  | CipherSuite Kex_RSA None (MACOnly SHA256)                            -> Correct TLS_RSA_WITH_NULL_SHA256
+  | CipherSuite Kex_RSA None (MtE (Stream RC4_128) MD5)                  -> Correct TLS_RSA_WITH_RC4_128_MD5
+  | CipherSuite Kex_RSA None (MtE (Stream RC4_128) SHA1)                 -> Correct TLS_RSA_WITH_RC4_128_SHA
+  | CipherSuite Kex_RSA None (MtE (Block TDES_EDE_CBC) SHA1)             -> Correct TLS_RSA_WITH_3DES_EDE_CBC_SHA
+  | CipherSuite Kex_RSA None (MtE (Block AES_128_CBC) SHA1)              -> Correct TLS_RSA_WITH_AES_128_CBC_SHA
+  | CipherSuite Kex_RSA None (MtE (Block AES_256_CBC) SHA1)              -> Correct TLS_RSA_WITH_AES_256_CBC_SHA
+  | CipherSuite Kex_RSA None (MtE (Block AES_128_CBC) SHA256)            -> Correct TLS_RSA_WITH_AES_128_CBC_SHA256
+  | CipherSuite Kex_RSA None (MtE (Block AES_256_CBC) SHA256)            -> Correct TLS_RSA_WITH_AES_256_CBC_SHA256
 
-    | CipherSuite Kex_DHE (Some DSA) (MtE (Block TDES_EDE_CBC) SHA1)    ->  Correct TLS_DHE_DSS_WITH_3DES_EDE_CBC_SHA
-    | CipherSuite Kex_DHE (Some RSASIG) (MtE (Block TDES_EDE_CBC) SHA1)    ->  Correct TLS_DHE_RSA_WITH_3DES_EDE_CBC_SHA
-    | CipherSuite Kex_DHE (Some DSA) (MtE (Block AES_128_CBC) SHA1)     ->  Correct TLS_DHE_DSS_WITH_AES_128_CBC_SHA
-    | CipherSuite Kex_DHE (Some RSASIG) (MtE (Block AES_128_CBC) SHA1)     ->  Correct TLS_DHE_RSA_WITH_AES_128_CBC_SHA
-    | CipherSuite Kex_DHE (Some DSA) (MtE (Block AES_256_CBC) SHA1)     ->  Correct TLS_DHE_DSS_WITH_AES_256_CBC_SHA
-    | CipherSuite Kex_DHE (Some RSASIG) (MtE (Block AES_256_CBC) SHA1)     ->  Correct TLS_DHE_RSA_WITH_AES_256_CBC_SHA
-    | CipherSuite Kex_DHE (Some DSA) (MtE (Block AES_128_CBC) SHA256)  ->  Correct TLS_DHE_DSS_WITH_AES_128_CBC_SHA256
-    | CipherSuite Kex_DHE (Some RSASIG) (MtE (Block AES_128_CBC) SHA256)  ->  Correct TLS_DHE_RSA_WITH_AES_128_CBC_SHA256
-    | CipherSuite Kex_DHE (Some DSA) (MtE (Block AES_256_CBC) SHA256)  ->  Correct TLS_DHE_DSS_WITH_AES_256_CBC_SHA256
-    | CipherSuite Kex_DHE (Some RSASIG) (MtE (Block AES_256_CBC) SHA256)  ->  Correct TLS_DHE_RSA_WITH_AES_256_CBC_SHA256
+  | CipherSuite Kex_DHE (Some DSA)    (MtE (Block TDES_EDE_CBC) SHA1)    -> Correct TLS_DHE_DSS_WITH_3DES_EDE_CBC_SHA
+  | CipherSuite Kex_DHE (Some RSASIG) (MtE (Block TDES_EDE_CBC) SHA1)    -> Correct TLS_DHE_RSA_WITH_3DES_EDE_CBC_SHA
+  | CipherSuite Kex_DHE (Some DSA)    (MtE (Block AES_128_CBC) SHA1)     -> Correct TLS_DHE_DSS_WITH_AES_128_CBC_SHA
+  | CipherSuite Kex_DHE (Some RSASIG) (MtE (Block AES_128_CBC) SHA1)     -> Correct TLS_DHE_RSA_WITH_AES_128_CBC_SHA
+  | CipherSuite Kex_DHE (Some DSA)    (MtE (Block AES_256_CBC) SHA1)     -> Correct TLS_DHE_DSS_WITH_AES_256_CBC_SHA
+  | CipherSuite Kex_DHE (Some RSASIG) (MtE (Block AES_256_CBC) SHA1)     -> Correct TLS_DHE_RSA_WITH_AES_256_CBC_SHA
+  | CipherSuite Kex_DHE (Some DSA)    (MtE (Block AES_128_CBC) SHA256)   -> Correct TLS_DHE_DSS_WITH_AES_128_CBC_SHA256
+  | CipherSuite Kex_DHE (Some RSASIG) (MtE (Block AES_128_CBC) SHA256)   -> Correct TLS_DHE_RSA_WITH_AES_128_CBC_SHA256
+  | CipherSuite Kex_DHE (Some DSA)    (MtE (Block AES_256_CBC) SHA256)   -> Correct TLS_DHE_DSS_WITH_AES_256_CBC_SHA256
+  | CipherSuite Kex_DHE (Some RSASIG) (MtE (Block AES_256_CBC) SHA256)   -> Correct TLS_DHE_RSA_WITH_AES_256_CBC_SHA256
 
-    | CipherSuite Kex_ECDHE (Some RSASIG) (MtE (Stream RC4_128) SHA1)       ->  Correct TLS_ECDHE_RSA_WITH_RC4_128_SHA
-    | CipherSuite Kex_ECDHE (Some RSASIG) (MtE (Block TDES_EDE_CBC) SHA1)  ->  Correct TLS_ECDHE_RSA_WITH_3DES_EDE_CBC_SHA
-    | CipherSuite Kex_ECDHE (Some RSASIG) (MtE (Block AES_128_CBC) SHA1)   ->  Correct TLS_ECDHE_RSA_WITH_AES_128_CBC_SHA
-    | CipherSuite Kex_ECDHE (Some RSASIG) (MtE (Block AES_128_CBC) SHA256) -> Correct TLS_ECDHE_RSA_WITH_AES_128_CBC_SHA256
-    | CipherSuite Kex_ECDHE (Some RSASIG) (MtE (Block AES_256_CBC) SHA1)    ->  Correct TLS_ECDHE_RSA_WITH_AES_256_CBC_SHA
-    | CipherSuite Kex_ECDHE (Some RSASIG) (MtE (Block AES_256_CBC) SHA384) -> Correct TLS_ECDHE_RSA_WITH_AES_256_CBC_SHA384
+  | CipherSuite Kex_ECDHE (Some RSASIG) (MtE (Stream RC4_128) SHA1)      -> Correct TLS_ECDHE_RSA_WITH_RC4_128_SHA
+  | CipherSuite Kex_ECDHE (Some RSASIG) (MtE (Block TDES_EDE_CBC) SHA1)  -> Correct TLS_ECDHE_RSA_WITH_3DES_EDE_CBC_SHA
+  | CipherSuite Kex_ECDHE (Some RSASIG) (MtE (Block AES_128_CBC) SHA1)   -> Correct TLS_ECDHE_RSA_WITH_AES_128_CBC_SHA
+  | CipherSuite Kex_ECDHE (Some RSASIG) (MtE (Block AES_128_CBC) SHA256) -> Correct TLS_ECDHE_RSA_WITH_AES_128_CBC_SHA256
+  | CipherSuite Kex_ECDHE (Some RSASIG) (MtE (Block AES_256_CBC) SHA1)   -> Correct TLS_ECDHE_RSA_WITH_AES_256_CBC_SHA
+  | CipherSuite Kex_ECDHE (Some RSASIG) (MtE (Block AES_256_CBC) SHA384) -> Correct TLS_ECDHE_RSA_WITH_AES_256_CBC_SHA384
 
-    | CipherSuite Kex_ECDHE (Some RSASIG) (AEAD AES_128_GCM SHA256) -> Correct TLS_ECDHE_RSA_WITH_AES_128_GCM_SHA256
-    | CipherSuite Kex_ECDHE (Some RSASIG) (AEAD AES_256_GCM SHA384) -> Correct TLS_ECDHE_RSA_WITH_AES_256_GCM_SHA384
+  | CipherSuite Kex_ECDHE (Some RSASIG) (AEAD AES_128_GCM SHA256)        -> Correct TLS_ECDHE_RSA_WITH_AES_128_GCM_SHA256
+  | CipherSuite Kex_ECDHE (Some RSASIG) (AEAD AES_256_GCM SHA384)        -> Correct TLS_ECDHE_RSA_WITH_AES_256_GCM_SHA384
 
-    | CipherSuite Kex_DHE None (MtE (Stream RC4_128) MD5)         ->  Correct TLS_DH_anon_WITH_RC4_128_MD5
-    | CipherSuite Kex_DHE None (MtE (Block TDES_EDE_CBC) SHA1)    ->  Correct TLS_DH_anon_WITH_3DES_EDE_CBC_SHA
-    | CipherSuite Kex_DHE None (MtE (Block AES_128_CBC) SHA1)     ->  Correct TLS_DH_anon_WITH_AES_128_CBC_SHA
-    | CipherSuite Kex_DHE None (MtE (Block AES_256_CBC) SHA1)     ->  Correct TLS_DH_anon_WITH_AES_256_CBC_SHA
-    | CipherSuite Kex_DHE None (MtE (Block AES_128_CBC) SHA256)  ->  Correct TLS_DH_anon_WITH_AES_128_CBC_SHA256
-    | CipherSuite Kex_DHE None (MtE (Block AES_256_CBC) SHA256)  ->  Correct TLS_DH_anon_WITH_AES_256_CBC_SHA256
+  | CipherSuite Kex_DHE None (MtE (Stream RC4_128) MD5)                  -> Correct TLS_DH_anon_WITH_RC4_128_MD5
+  | CipherSuite Kex_DHE None (MtE (Block TDES_EDE_CBC) SHA1)             -> Correct TLS_DH_anon_WITH_3DES_EDE_CBC_SHA
+  | CipherSuite Kex_DHE None (MtE (Block AES_128_CBC) SHA1)              -> Correct TLS_DH_anon_WITH_AES_128_CBC_SHA
+  | CipherSuite Kex_DHE None (MtE (Block AES_256_CBC) SHA1)              -> Correct TLS_DH_anon_WITH_AES_256_CBC_SHA
+  | CipherSuite Kex_DHE None (MtE (Block AES_128_CBC) SHA256)            -> Correct TLS_DH_anon_WITH_AES_128_CBC_SHA256
+  | CipherSuite Kex_DHE None (MtE (Block AES_256_CBC) SHA256)            -> Correct TLS_DH_anon_WITH_AES_256_CBC_SHA256
 
-    | CipherSuite Kex_RSA None     (AEAD AES_128_GCM SHA256)  ->  Correct TLS_RSA_WITH_AES_128_GCM_SHA256
-    | CipherSuite Kex_RSA None     (AEAD AES_256_GCM SHA384)  ->  Correct TLS_RSA_WITH_AES_256_GCM_SHA384
-    | CipherSuite Kex_DHE (Some RSASIG) (AEAD AES_128_GCM SHA256)  ->  Correct TLS_DHE_RSA_WITH_AES_128_GCM_SHA256
-    | CipherSuite Kex_DHE (Some RSASIG) (AEAD AES_256_GCM SHA384)  ->  Correct TLS_DHE_RSA_WITH_AES_256_GCM_SHA384
-    | CipherSuite Kex_DH (Some RSASIG)  (AEAD AES_128_GCM SHA256)  ->  Correct TLS_DH_RSA_WITH_AES_128_GCM_SHA256
-    | CipherSuite Kex_DH (Some RSASIG)  (AEAD AES_256_GCM SHA384)  ->  Correct TLS_DH_RSA_WITH_AES_256_GCM_SHA384
-    | CipherSuite Kex_DHE (Some DSA) (AEAD AES_128_GCM SHA256)  ->  Correct TLS_DHE_DSS_WITH_AES_128_GCM_SHA256
-    | CipherSuite Kex_DHE (Some DSA) (AEAD AES_256_GCM SHA384)  ->  Correct TLS_DHE_DSS_WITH_AES_256_GCM_SHA384
-    | CipherSuite Kex_DH (Some DSA)  (AEAD AES_128_GCM SHA256)  ->  Correct TLS_DH_DSS_WITH_AES_128_GCM_SHA256
-    | CipherSuite Kex_DH (Some DSA)  (AEAD AES_256_GCM SHA384)  ->  Correct TLS_DH_DSS_WITH_AES_256_GCM_SHA384
-    | CipherSuite Kex_DHE None (AEAD AES_128_GCM SHA256)  ->  Correct TLS_DH_anon_WITH_AES_128_GCM_SHA256
-    | CipherSuite Kex_DHE None (AEAD AES_256_GCM SHA384)  ->  Correct TLS_DH_anon_WITH_AES_256_GCM_SHA384
+  | CipherSuite Kex_RSA None          (AEAD AES_128_GCM SHA256)          -> Correct TLS_RSA_WITH_AES_128_GCM_SHA256
+  | CipherSuite Kex_RSA None          (AEAD AES_256_GCM SHA384)          -> Correct TLS_RSA_WITH_AES_256_GCM_SHA384
+  | CipherSuite Kex_DHE (Some RSASIG) (AEAD AES_128_GCM SHA256)          -> Correct TLS_DHE_RSA_WITH_AES_128_GCM_SHA256
+  | CipherSuite Kex_DHE (Some RSASIG) (AEAD AES_256_GCM SHA384)          -> Correct TLS_DHE_RSA_WITH_AES_256_GCM_SHA384
+  | CipherSuite Kex_DH  (Some RSASIG) (AEAD AES_128_GCM SHA256)          -> Correct TLS_DH_RSA_WITH_AES_128_GCM_SHA256
+  | CipherSuite Kex_DH  (Some RSASIG) (AEAD AES_256_GCM SHA384)          -> Correct TLS_DH_RSA_WITH_AES_256_GCM_SHA384
+  | CipherSuite Kex_DHE (Some DSA)    (AEAD AES_128_GCM SHA256)          -> Correct TLS_DHE_DSS_WITH_AES_128_GCM_SHA256
+  | CipherSuite Kex_DHE (Some DSA)    (AEAD AES_256_GCM SHA384)          -> Correct TLS_DHE_DSS_WITH_AES_256_GCM_SHA384
+  | CipherSuite Kex_DH  (Some DSA)    (AEAD AES_128_GCM SHA256)          -> Correct TLS_DH_DSS_WITH_AES_128_GCM_SHA256
+  | CipherSuite Kex_DH  (Some DSA)    (AEAD AES_256_GCM SHA384)          -> Correct TLS_DH_DSS_WITH_AES_256_GCM_SHA384
+  | CipherSuite Kex_DHE None          (AEAD AES_128_GCM SHA256)          -> Correct TLS_DH_anon_WITH_AES_128_GCM_SHA256
+  | CipherSuite Kex_DHE None          (AEAD AES_256_GCM SHA384)          -> Correct TLS_DH_anon_WITH_AES_256_GCM_SHA384
 
-    | _ -> Error(AD_illegal_parameter, perror __SOURCE_FILE__ __LINE__ "Invoked on a unknown ciphersuite")
+  | _ -> Error(AD_illegal_parameter, perror __SOURCE_FILE__ __LINE__ "Invoked on a unknown ciphersuite")
 
 #set-options "--max_ifuel 5 --initial_ifuel 5 --max_fuel 1 --initial_fuel 1"
 
 val names_of_cipherSuites : cipherSuites -> Tot (result cipherSuiteNames)
 let rec names_of_cipherSuites css =
-    match css with
-    | [] -> Correct []
-    | h::t ->
-       begin match name_of_cipherSuite h with
-             | Error(x,y) -> Error(x,y)
-             | Correct(n) ->
-                begin match names_of_cipherSuites t with
-                      | Error(x,y) -> Error(x,y)
-                      | Correct(rem) -> Correct (n::rem)
-                end
-       end
+  match css with
+  | [] -> Correct []
+  | h::t ->
+    begin
+    match name_of_cipherSuite h with
+    | Error(x,y) -> Error(x,y)
+    | Correct n  ->
+      begin
+	match names_of_cipherSuites t with
+        | Error(x,y)  -> Error(x,y)
+        | Correct rem -> Correct (n::rem)
+      end
+    end
 
 // migrated contentType to Content.fst (this is internal to TLS)
 
 val bytes_of_seq: n:nat{ repr_bytes n <= 8 } -> Tot bytes
 let bytes_of_seq sn = bytes_of_int 8 sn
+
 val seq_of_bytes: b:bytes{ length b <= 8 } -> Tot nat
 let seq_of_bytes b = int_of_bytes b
 
 val vlbytes: lSize:nat -> b:bytes{repr_bytes (length b) <= lSize} -> Tot (r:bytes{length r = lSize + length b})
 let vlbytes lSize b = bytes_of_int lSize (length b) @| b
 
+val lemma_vlbytes_len : i:nat -> b:bytes{repr_bytes (length b) <= i}
+  -> Lemma (ensures (length (vlbytes i b) = i + length b))
+let lemma_vlbytes_len i b = ()
+
 val lemma_vlbytes_inj : i:nat
-          -> b:bytes{repr_bytes (length b) <= i}
-          -> b':bytes{repr_bytes (length b') <= i}
-          -> Lemma (requires (Seq.equal (vlbytes i b) (vlbytes i b')))
-                   (ensures (b=b'))
+  -> b:bytes{repr_bytes (length b) <= i}
+  -> b':bytes{repr_bytes (length b') <= i}
+  -> Lemma (requires (Seq.equal (vlbytes i b) (vlbytes i b')))
+          (ensures (b = b'))
 let lemma_vlbytes_inj i b b' =
   let l = bytes_of_int i (length b) in
   SeqProperties.lemma_append_inj l b l b'
@@ -868,43 +892,48 @@ let vlsplit lSize vlb =
   then Correct(Platform.Bytes.split b l)
   else Error(AD_decode_error, perror __SOURCE_FILE__ __LINE__ "")
 
-val vlparse: lSize:nat{lSize <= 4} -> vlb:bytes //{lSize <= length vlb}
-             -> Tot (result (b:bytes{repr_bytes (length b) <= lSize /\ Seq.equal vlb (vlbytes lSize b)}))
+val vlparse: lSize:nat{lSize <= 4} -> vlb:bytes{lSize <= length vlb}
+  -> Tot (result (b:bytes{repr_bytes (length b) <= lSize /\ Seq.equal vlb (vlbytes lSize b)}))
 let vlparse lSize vlb =
-    if lSize <= length vlb then
-      let (vl,b) = Platform.Bytes.split vlb lSize in
-      let l = int_of_bytes vl in
-      if l = length b
-      then Correct b
-      else Error(AD_decode_error, perror __SOURCE_FILE__ __LINE__ "")
-    else Error(AD_decode_error, perror __SOURCE_FILE__ __LINE__ "")
+  let vl,b = split vlb lSize in
+  if int_of_bytes vl = length b
+  then Correct b
+  else Error(AD_decode_error, perror __SOURCE_FILE__ __LINE__ "")
 
-val lemma_vlbytes_len : i:nat -> b:bytes{repr_bytes (length b) <= i}
-                        -> Lemma (ensures (length (vlbytes i b) = i + length b))
-let lemma_vlbytes_len i b = ()
+val vlparse_vlbytes: lSize:nat{lSize <= 4} -> vlb:bytes{repr_bytes (length vlb) <= lSize} -> Lemma 
+  (requires (True))
+  (ensures (vlparse lSize (vlbytes lSize vlb) = Correct vlb))
+  [SMTPat (vlparse lSize (vlbytes lSize vlb))]
+let vlparse_vlbytes lSize vlb =
+  let vl,b = split (vlbytes lSize vlb) lSize in
+  assert (Seq.equal vl (bytes_of_int lSize (length vlb)));
+  int_of_bytes_of_int lSize (length vlb);
+  match vlparse lSize (vlbytes lSize vlb) with
+  | Error z   -> ()
+  | Correct b -> lemma_vlbytes_inj lSize vlb b
 
 type certType =
-    | RSA_sign
-    | DSA_sign
-    | RSA_fixed_dh
-    | DSA_fixed_dh
+  | RSA_sign
+  | DSA_sign
+  | RSA_fixed_dh
+  | DSA_fixed_dh
 
-val certTypeBytes : certType -> Tot (lbytes 1)
+val certTypeBytes: certType -> Tot (lbytes 1)
 let certTypeBytes ct =
-    match ct with
-    | RSA_sign     -> abyte (1z)
-    | DSA_sign     -> abyte (2z)
-    | RSA_fixed_dh -> abyte (3z)
-    | DSA_fixed_dh -> abyte (4z)
+  match ct with
+  | RSA_sign     -> abyte 1z
+  | DSA_sign     -> abyte 2z
+  | RSA_fixed_dh -> abyte 3z
+  | DSA_fixed_dh -> abyte 4z
 
 val parseCertType: pinverse_t certTypeBytes
 let parseCertType b =
-    match cbyte b with
-    | (1z) -> Correct(RSA_sign)
-    | (2z) -> Correct(DSA_sign)
-    | (3z) -> Correct(RSA_fixed_dh)
-    | (4z) -> Correct(DSA_fixed_dh)
-    | _ -> Error(AD_decode_error, perror __SOURCE_FILE__ __LINE__ "")
+  match cbyte b with
+  | 1z -> Correct RSA_sign
+  | 2z -> Correct DSA_sign
+  | 3z -> Correct RSA_fixed_dh
+  | 4z -> Correct DSA_fixed_dh
+  | _ -> Error(AD_decode_error, perror __SOURCE_FILE__ __LINE__ "")
 
 val inverse_certType: x:_ -> Lemma
   (requires (True))
@@ -921,24 +950,23 @@ let pinverse_certType x = ()
 #set-options "--max_fuel 1 --initial_fuel 1"
 val certificateTypeListBytes: ctl:list certType -> Tot (lbytes (List.Tot.length ctl))
 let rec certificateTypeListBytes ctl =
-    match ctl with
-    | [] -> empty_bytes
-    | h::t ->
-        let ct = certTypeBytes h in
-        ct @| certificateTypeListBytes t
+  match ctl with
+  | [] -> empty_bytes
+  | h::t ->
+    let ct = certTypeBytes h in
+    ct @| certificateTypeListBytes t
 
 val parseCertificateTypeList: data:bytes -> Tot (list certType) (decreases (length data))
 let rec parseCertificateTypeList data =
-  let l = length data in
-    if l = 0 then []
-    else
-        let (thisByte,data) = Platform.Bytes.split data 1 in
-        match parseCertType thisByte with
-        | Error(z) -> // we skip this one
-            parseCertificateTypeList data
-        | Correct(ct) ->
-            let rem = parseCertificateTypeList data in
-            ct :: rem
+  if length data = 0 then []
+  else
+    let (thisByte,data) = Platform.Bytes.split data 1 in
+    match parseCertType thisByte with
+    | Error z -> // we skip this one
+      parseCertificateTypeList data
+    | Correct ct ->
+      let rem = parseCertificateTypeList data in
+      ct :: rem
 
 #set-options "--max_ifuel 4 --initial_ifuel 1 --max_fuel 4 --initial_fuel 1"
 
@@ -947,45 +975,49 @@ let defaultCertTypes sign cs =
   let alg = sigAlg_of_ciphersuite cs in
     if sign then
       match alg with
-        | RSASIG -> [RSA_sign]
-        | DSA -> [DSA_sign]
-        | _ -> unexpected "[defaultCertTypes] invoked on an invalid ciphersuite"
+      | RSASIG -> [RSA_sign]
+      | DSA -> [DSA_sign]
+      | _ -> unexpected "[defaultCertTypes] invoked on an invalid ciphersuite"
     else
       match alg with
-        | RSASIG -> [RSA_fixed_dh]
-        | DSA -> [DSA_fixed_dh]
-        | _ -> unexpected "[defaultCertTypes] invoked on an invalid ciphersuite"
+      | RSASIG -> [RSA_fixed_dh]
+      | DSA -> [DSA_fixed_dh]
+      | _ -> unexpected "[defaultCertTypes] invoked on an invalid ciphersuite"
+
+#set-options "--max_ifuel 2 --initial_ifuel 2 --max_fuel 1 --initial_fuel 1"
 
 type dn = s:string{length(utf8 s) <= 256}
-val distinguishedNameListBytes: names:list dn -> Tot (b:bytes{length b <= op_Multiply 258  (List.Tot.length names)})
+
+val distinguishedNameListBytes: names:list dn -> Tot (b:bytes{length b <= op_Multiply 258 (List.Tot.length names)})
 let rec distinguishedNameListBytes names =
-    match names with
-    | [] -> empty_bytes
-    | h::t ->
-        lemma_repr_bytes_values (length (utf8 h));
-        let name = vlbytes 2 (utf8 h) in
-        name @| distinguishedNameListBytes t
+  match names with
+  | [] -> empty_bytes
+  | h::t ->
+    lemma_repr_bytes_values (length (utf8 h));
+    let name = vlbytes 2 (utf8 h) in
+    name @| distinguishedNameListBytes t
 
 val parseDistinguishedNameList: data:bytes -> res:list string -> Tot (result (list string)) (decreases (length data))
 let rec parseDistinguishedNameList data res =
-    if length data = 0 then
-        Correct (res)
+  if length data = 0 then
+    Correct res
+  else
+    if length data < 2 then
+      Error(AD_decode_error, perror __SOURCE_FILE__ __LINE__ "")
     else
-        if length data < 2 then
-            Error(AD_decode_error, perror __SOURCE_FILE__ __LINE__ "")
-        else
-            match vlsplit 2 data with
-            | Error(z) -> Error(z)
-            | Correct (nameBytes,data) ->
-               begin match iutf8_opt nameBytes with
-                     | None -> Error(AD_decode_error, perror __SOURCE_FILE__ __LINE__ "")
-                     | Some name ->
-                        let res = name :: res in
-                        parseDistinguishedNameList data res
-               end
+      match vlsplit 2 data with
+      | Error z -> Error z
+      | Correct (nameBytes,data) ->
+        begin
+	match iutf8_opt nameBytes with
+        | None -> Error(AD_decode_error, perror __SOURCE_FILE__ __LINE__ "")
+        | Some name ->
+          let res = name :: res in
+          parseDistinguishedNameList data res
+        end
 
 let contains_TLS_EMPTY_RENEGOTIATION_INFO_SCSV (css: list cipherSuite) =
-    List.Tot.mem (SCSV (TLS_EMPTY_RENEGOTIATION_INFO_SCSV)) css
+  List.Tot.mem (SCSV (TLS_EMPTY_RENEGOTIATION_INFO_SCSV)) css
 
 
 (* TODO: move all the definitions below to a separate file / figure out whether
@@ -1000,94 +1032,133 @@ type ffdhe =
   | FFDHE6144
   | FFDHE8192
 
+let _FFz = 0xFFz // Workaround for #514
+
 (* TLS 1.3 constants *)
 type namedGroup =
   | SEC of CoreCrypto.ec_curve
-  | EC_UNSUPPORTED of byte
+  | EC_UNSUPPORTED of (b:byte{b <> 0x17z /\ b <> 0x18z /\ b <> 0x19z})
   | FFDHE of ffdhe
-  | FFDHE_PRIVATE_USE of byte // fist byte is fixed
-  | ECDHE_PRIVATE_USE of byte // fist byte is fixed
-
+  | FFDHE_PRIVATE_USE of (b:byte{b = 0xFCz \/ b = 0xFDz \/ b = 0xFEz \/ b = _FFz})
+  | ECDHE_PRIVATE_USE of byte
+  
 val namedGroupBytes: namedGroup -> Tot (lbytes 2)
 let namedGroupBytes ng =
   match ng with
   | SEC ec ->
-    (match ec with
-    | ECC_P256                      -> abyte2 (0x00z, 0x17z)
-    | ECC_P384                      -> abyte2 (0x00z, 0x18z)
-    | ECC_P521                      -> abyte2 (0x00z, 0x19z))
-  | EC_UNSUPPORTED(b)               -> abyte2 (0x00z, b)
+    begin
+    match ec with
+    | ECC_P256		-> abyte2 (0x00z, 0x17z)
+    | ECC_P384		-> abyte2 (0x00z, 0x18z)
+    | ECC_P521		-> abyte2 (0x00z, 0x19z)
+    end
+  | EC_UNSUPPORTED b	-> abyte2 (0x00z, b)
   | FFDHE dhe ->
-    (match dhe with
-    | FFDHE2048                     -> abyte2 (0x01z, 0x00z)
-    | FFDHE3072                     -> abyte2 (0x01z, 0x01z)
-    | FFDHE4096                     -> abyte2 (0x01z, 0x02z)
-    | FFDHE6144                     -> abyte2 (0x01z, 0x03z)
-    | FFDHE8192                     -> abyte2 (0x01z, 0x04z)
-  )
-  | FFDHE_PRIVATE_USE(b)            -> abyte2 (0x01z, b)
-  | ECDHE_PRIVATE_USE(b)            -> abyte2 (0xFEz, b)
+    begin
+    match dhe with
+    | FFDHE2048		-> abyte2 (0x01z, 0x00z)
+    | FFDHE3072		-> abyte2 (0x01z, 0x01z)
+    | FFDHE4096		-> abyte2 (0x01z, 0x02z)
+    | FFDHE6144		-> abyte2 (0x01z, 0x03z)
+    | FFDHE8192		-> abyte2 (0x01z, 0x04z)
+    end
+  | FFDHE_PRIVATE_USE b -> abyte2 (0x01z, b)
+  | ECDHE_PRIVATE_USE b -> abyte2 (0xFEz, b)
 
 val parseNamedGroup: pinverse_t namedGroupBytes
 let parseNamedGroup b =
   match cbyte2 b with
-  | (0x00z, 0x17z) -> Correct (SEC(ECC_P256))
-  | (0x00z, 0x18z) -> Correct (SEC(ECC_P384))
-  | (0x00z, 0x19z) -> Correct (SEC(ECC_P521))
-  | (0x00z, x) -> let v = int_of_bytes (abyte x) in
-		   (*if v > 0 && v < 17 then *) Correct(EC_UNSUPPORTED (x))
-//		   else Error (AD_decode_error, perror __SOURCE_FILE__ __LINE__ "Wrong ec named group")
-  | (0x01z, 0x00z) -> Correct (FFDHE(FFDHE2048))
-  | (0x01z, 0x01z) -> Correct (FFDHE(FFDHE3072))
-  | (0x01z, 0x02z) -> Correct (FFDHE(FFDHE4096))
-  | (0x01z, 0x03z) -> Correct (FFDHE(FFDHE6144))
-  | (0x01z, 0x04z) -> Correct (FFDHE(FFDHE8192))
-  | (0x01z, v)      -> if v = 0xFCz || v = 0xFDz || v = 0xFEz || v = 0xFFz
-			then Correct (FFDHE_PRIVATE_USE v)
-			else Error (AD_decode_error, perror __SOURCE_FILE__ __LINE__ "Wrong ffdhe private use group")
-  | (0xFEz, v)      -> Correct (ECDHE_PRIVATE_USE v)
+  | (0x00z, 0x17z) -> Correct (SEC ECC_P256)
+  | (0x00z, 0x18z) -> Correct (SEC ECC_P384)
+  | (0x00z, 0x19z) -> Correct (SEC ECC_P521)
+  | (0x00z, b)     -> Correct (EC_UNSUPPORTED b) // REMARK: only values 0x01z-0x16z and 0x1Az-0x1Ez are assigned
+  | (0x01z, 0x00z) -> Correct (FFDHE FFDHE2048)
+  | (0x01z, 0x01z) -> Correct (FFDHE FFDHE3072)
+  | (0x01z, 0x02z) -> Correct (FFDHE FFDHE4096)
+  | (0x01z, 0x03z) -> Correct (FFDHE FFDHE6144)
+  | (0x01z, 0x04z) -> Correct (FFDHE FFDHE8192)
+  | (0x01z, b)     ->
+    if b = 0xFCz || b = 0xFDz || b = 0xFEz || b = 0xFFz
+    then Correct (FFDHE_PRIVATE_USE b)
+    else Error (AD_decode_error, perror __SOURCE_FILE__ __LINE__ "Wrong ffdhe private use group")
+  | (0xFEz, b)     -> Correct (ECDHE_PRIVATE_USE b)
   | _ -> Error (AD_decode_error, perror __SOURCE_FILE__ __LINE__ "Wrong named group")
 
+val inverse_namedGroup: x:_ -> Lemma
+  (requires (True))
+  (ensures lemma_inverse_g_f namedGroupBytes parseNamedGroup x)
+  [SMTPat (parseNamedGroup (namedGroupBytes x))]
+let inverse_namedGroup x = ()
 
-private val namedGroupsBytes0: groups:list namedGroup -> Tot (b:bytes { length b = op_Multiply 2 (List.Tot.length groups)})
+val pinverse_namedGroup: x:_ -> Lemma
+  (requires (True))
+  (ensures (lemma_pinverse_f_g Seq.equal namedGroupBytes parseNamedGroup x))
+  [SMTPat (namedGroupBytes (Correct._0 (parseNamedGroup x)))]
+let pinverse_namedGroup x = ()
+
+
+private val namedGroupsBytes0: groups:list namedGroup
+  -> Tot (b:bytes { length b = op_Multiply 2 (List.Tot.length groups)})
 let rec namedGroupsBytes0 groups =
   match groups with
   | [] -> empty_bytes
   | g::gs -> namedGroupBytes g @| namedGroupsBytes0 gs
 
-val namedGroupsBytes: groups:list namedGroup{List.Tot.length groups < 65536/2}-> Tot (b:bytes { length b = 2 + op_Multiply 2 (List.Tot.length groups)})
+val namedGroupsBytes: groups:list namedGroup{List.Tot.length groups < 65536/2}
+  -> Tot (b:bytes { length b = 2 + op_Multiply 2 (List.Tot.length groups)})
 let namedGroupsBytes groups =
   let gs = namedGroupsBytes0 groups in
   lemma_repr_bytes_values (length gs);
   vlbytes 2 gs
+  
+private val parseNamedGroups0: b:bytes -> l:list namedGroup 
+  -> Tot (result (groups:list namedGroup{List.Tot.length groups = List.Tot.length l + length b / 2}))
+  (decreases (length b))
+let rec parseNamedGroups0 b groups =
+  if length b > 0 then
+    if length b >= 2 then
+      let (ng, bytes) = split b 2 in
+      match parseNamedGroup ng with
+      | Correct ng -> parseNamedGroups0 bytes (ng::groups)
+      | Error z    -> Error z
+    else Error (AD_decode_error, perror __SOURCE_FILE__ __LINE__ "")
+  else Correct groups
 
-//val parseNamedGroups: pinverse_t namedGroupsBytes
-let parseNamedGroups (b:bytes) =
-  let rec (aux: b:bytes -> list namedGroup -> Tot (result (list namedGroup)) (decreases (length b))) = fun b groups ->
-    if length b > 0 then
-      if length b >= 2 then
-	let (ng, bytes) = split b 2 in
-	match parseNamedGroup ng with
-	| Correct(ng) -> aux bytes (ng::groups)
-	| Error(z) -> Error(z)
-      else Error (AD_decode_error, perror __SOURCE_FILE__ __LINE__ "")
-    else Correct(groups) in
+val parseNamedGroups: b:bytes { 2 <= length b /\ length b < 65538 }
+  -> Tot (result (groups:list namedGroup{List.Tot.length groups = (length b - 2) / 2}))
+let parseNamedGroups b =
   match vlparse 2 b with
-  | Correct(b) -> aux b []
-  | Error(z) -> Error(AD_decode_error, perror __SOURCE_FILE__ __LINE__ "Failed to parse named groups")
+  | Correct b -> parseNamedGroups0 b []
+  | Error z   ->
+    Error(AD_decode_error, perror __SOURCE_FILE__ __LINE__ "Failed to parse named groups")
 
 
-(* TODO : precise configurationId type *)
-type configurationId = b:bytes{not (equalBytes b empty_bytes) /\ length b < 65536}
+type configurationId = b:bytes{0 < length b /\ length b < 65536}
 
-val configurationIdBytes: configurationId -> Tot bytes
+val configurationIdBytes: configurationId -> Tot (b:bytes{2 < length b /\ length b < 65538})
 let configurationIdBytes cid =
   lemma_repr_bytes_values (length cid);
   vlbytes 2 cid
 
-//val parseConfigurationId: pinverse_t configurationIdBytes
+val parseConfigurationId: pinverse_t configurationIdBytes
 let parseConfigurationId b =
-  vlparse 2 b
+  match vlparse 2 b with
+  | Error z -> Error z
+  | Correct b -> Correct b
+
+val inverse_configurationId: x:_ -> Lemma
+  (requires (True))
+  (ensures lemma_inverse_g_f configurationIdBytes parseConfigurationId x)
+  [SMTPat (parseConfigurationId (configurationIdBytes x))]
+let inverse_configurationId x =
+  lemma_repr_bytes_values (length x)
+
+val pinverse_configurationId: x:_ -> Lemma
+  (requires (True))
+  (ensures (lemma_pinverse_f_g Seq.equal configurationIdBytes parseConfigurationId x))
+  [SMTPat (configurationIdBytes (Correct._0 (parseConfigurationId x)))]
+let pinverse_configurationId x = ()
+
 
 type uint32 = b:lbytes 4
 
@@ -1099,31 +1170,57 @@ let parseUint32 b =
   if length b = 4 then Correct(b)
   else Error (AD_decode_error, perror __SOURCE_FILE__ __LINE__ "")
 
+val inverse_uint32: x:_ -> Lemma
+  (requires (True))
+  (ensures lemma_inverse_g_f uint32Bytes parseUint32 x)
+  [SMTPat (parseUint32 (uint32Bytes x))]
+let inverse_uint32 x = ()
+
+val pinverse_uint32: x:_ -> Lemma
+  (requires (True))
+  (ensures (lemma_pinverse_f_g Seq.equal uint32Bytes parseUint32 x))
+  [SMTPat (uint32Bytes (Correct._0 (parseUint32 x)))]
+let pinverse_uint32 x = ()
+
+
 type earlyDataType =
   | ClientAuthentication
   | EarlyData
   | ClientAuthenticationAndData
 
-val earlyDataTypeBytes : earlyDataType -> Tot (lbytes 1)
+val earlyDataTypeBytes: earlyDataType -> Tot (lbytes 1)
 let earlyDataTypeBytes edt =
   match edt with
-  | ClientAuthentication          -> abyte 1z
-  | EarlyData                     -> abyte 2z
-  | ClientAuthenticationAndData   -> abyte 3z
+  | ClientAuthentication        -> abyte 1z
+  | EarlyData                   -> abyte 2z
+  | ClientAuthenticationAndData -> abyte 3z
 
 val parseEarlyDataType: pinverse_t earlyDataTypeBytes
 let parseEarlyDataType b =
-    match cbyte b with
-    | (1z) -> Correct (ClientAuthentication)
-    | (2z) -> Correct (EarlyData)
-    | (3z) -> Correct (ClientAuthenticationAndData)
-    | _ -> Error (AD_decode_error, perror __SOURCE_FILE__ __LINE__ "Failed to parse early data type")
+  match cbyte b with
+  | 1z -> Correct ClientAuthentication
+  | 2z -> Correct EarlyData
+  | 3z -> Correct ClientAuthenticationAndData
+  | _  -> Error (AD_decode_error, perror __SOURCE_FILE__ __LINE__ "Failed to parse early data type")
+
+val inverse_earlyDataType: x:_ -> Lemma
+  (requires (True))
+  (ensures lemma_inverse_g_f earlyDataTypeBytes parseEarlyDataType x)
+  [SMTPat (parseEarlyDataType (earlyDataTypeBytes x))]
+let inverse_earlyDataType x = ()
+
+val pinverse_earlyDataType: x:_ -> Lemma
+  (requires (True))
+  (ensures (lemma_pinverse_f_g Seq.equal earlyDataTypeBytes parseEarlyDataType x))
+  [SMTPat (earlyDataTypeBytes (Correct._0 (parseEarlyDataType x)))]
+let pinverse_earlyDataType x = ()
 
 // TODO : replace with more precise types when available
 type configurationExtension =
   | UnknownConfigurationExtension:
       typ:lbytes 2 -> payload: bytes { repr_bytes (length payload) <= 2 } -> configurationExtension
 
+// Should we strengthen the result type to b:bytes{length b >= 4}?
 val configurationExtensionBytes: ce:configurationExtension -> Tot bytes
 let configurationExtensionBytes ce =
   match ce with
@@ -1132,18 +1229,48 @@ let configurationExtensionBytes ce =
 val parseConfigurationExtension: pinverse_t configurationExtensionBytes
 let parseConfigurationExtension b =
   if length b >= 4 then
-  ( let (typ, payload) = split b 2 in
+    let (typ,payload) = split b 2 in
     match vlparse 2 payload with
-    | Correct (payload) -> Correct (UnknownConfigurationExtension typ payload)
-    | Error(z) -> Error(z))
+    | Correct payload -> Correct (UnknownConfigurationExtension typ payload)
+    | Error z -> Error z
   else Error (AD_decode_error, perror __SOURCE_FILE__ __LINE__ "Too few bytes to parse a configuration extension")
+
+val inverse_configurationExtension: x:_ -> Lemma
+  (requires (True))
+  (ensures lemma_inverse_g_f configurationExtensionBytes parseConfigurationExtension x)
+  [SMTPat (parseConfigurationExtension (configurationExtensionBytes x))]
+let inverse_configurationExtension x =
+  match x with
+  | UnknownConfigurationExtension typ payload -> 
+  let b = typ @| vlbytes 2 payload in
+  let b0,b1 = split b 2 in
+  let vl,b = split b1 2 in
+  vlparse_vlbytes 2 b;
+  assert (Seq.equal vl (bytes_of_int 2 (length b)));
+  assert (Seq.equal b0 typ);
+  assert (Seq.equal b payload)
+ 
+val pinverse_configurationExtension: x:_ -> Lemma
+  (requires (True))
+  (ensures (lemma_pinverse_f_g Seq.equal configurationExtensionBytes parseConfigurationExtension x))
+  [SMTPat (configurationExtensionBytes (Correct._0 (parseConfigurationExtension x)))]
+let pinverse_configurationExtension x = ()
+
+// Choice: truncate when maximum length is exceeded
+// Non top-level let rec yields stack overflow during extraction
+let rec configurationExtensionsBytes_aux (b:bytes{length b < 65536}) (ces:list configurationExtension): Tot (b:bytes{length b < 65536}) (decreases ces) =
+  match ces with
+  | [] -> b
+  | ce::ces ->
+    if length (b @| configurationExtensionBytes ce) < 65536 then
+      configurationExtensionsBytes_aux (b @| configurationExtensionBytes ce) ces
+    else b
 
 val configurationExtensionsBytes: list configurationExtension -> Tot bytes
 let configurationExtensionsBytes ce =
-  let b = (List.Tot.fold_left (fun bytes x -> bytes @| configurationExtensionBytes x) empty_bytes ce) in
-  admit(); //TODO
+  let b = configurationExtensionsBytes_aux empty_bytes ce in
+  lemma_repr_bytes_values (length b);
   vlbytes 2 b
-
 
 val parseConfigurationExtensions: pinverse_t configurationExtensionsBytes
 let parseConfigurationExtensions b =
@@ -1168,103 +1295,153 @@ let parseConfigurationExtensions b =
   else Error(AD_decode_error, perror __SOURCE_FILE__ __LINE__ "Failed to parse configuration extension")
 
 
+type sigHashAlg = sigAlg * hashAlg'
+
 val sigHashAlgBytes: sigHashAlg -> Tot (lbytes 2)
 let sigHashAlgBytes sha =
   let sign = sigAlgBytes (fst sha) in
-  admit(); // FIXME
   let hash = hashAlgBytes (snd sha) in
   hash @| sign
 
 val parseSigHashAlg: pinverse_t sigHashAlgBytes
 let parseSigHashAlg b =
-  if length b = 2 then
-    let (hash, sign) = split b 1 in
-    match parseSigAlg sign with
-    | Correct(sign) ->
-	(match parseHashAlg hash with
-	| Correct(hash) -> Correct(sign, hash)
-	| Error(z) -> Error(z))
-    | Error(z) -> Error(z)
-  else Error (AD_decode_error, perror __SOURCE_FILE__ __LINE__ "Remaining unparsed bytes after signature hash algorithm")
+  let hash,sign = split b 1 in
+  match parseSigAlg sign with
+  | Correct sign ->
+    begin
+    match parseHashAlg hash with
+    | Correct hash -> Correct(sign, hash)
+    | Error z -> Error z
+    end
+  | Error z -> Error z
 
-val sigHashAlgsBytes: list sigHashAlg -> Tot bytes
+// Non top-level let rec yields stack overflow during extraction
+let rec sigHashAlgsBytes_aux (b:bytes) (algs:list sigHashAlg{length b + op_Multiply 2 (List.Tot.length algs) < 65536}) : Tot (r:bytes{length r < 65536}) (decreases algs) =
+  match algs with
+  | [] -> b
+  | alg::algs' -> sigHashAlgsBytes_aux (sigHashAlgBytes alg @| b) algs'
+  
+val sigHashAlgsBytes: algs:list sigHashAlg{List.Tot.length algs < 65536/2}
+  -> Tot (b:bytes{2 <= length b /\ length b < 65538})
 let sigHashAlgsBytes algs =
-  admit(); // TODO
-  vlbytes 2 (List.Tot.fold_left (fun l x -> sigHashAlgBytes x @| l) empty_bytes algs)
+  let b = sigHashAlgsBytes_aux empty_bytes algs in
+  lemma_repr_bytes_values (length b);
+  vlbytes 2 b
 
 val parseSigHashAlgs: pinverse_t sigHashAlgsBytes
 let parseSigHashAlgs b =
-  let rec (aux: b:bytes -> list sigHashAlg -> Tot (result (list sigHashAlg)) (decreases (length b))) = fun b algs ->
+  let rec aux: b:bytes -> algs:list sigHashAlg{length b + op_Multiply 2 (List.Tot.length algs) < 65536} -> Tot (result (l:list sigHashAlg{List.Tot.length l < 65536/2})) (decreases (length b)) = fun b algs ->
     if length b > 0 then
       if length b >= 2 then
-      let (alg, bytes) = split b 2 in
+      let alg,bytes = split b 2 in
       match parseSigHashAlg alg with
-      | Correct(sha) -> aux bytes (sha::algs)
-      | Error(z) -> Error(z)
+      | Correct sha -> aux bytes (sha::algs)
+      | Error z     -> Error z
       else Error (AD_decode_error, perror __SOURCE_FILE__ __LINE__ "Too few bytes to parse sig hash algs")
-    else Correct(algs) in
+    else Correct algs in
   match vlparse 2 b with
-  | Correct (b) -> aux b []
-  | Error(z) -> Error(AD_decode_error, perror __SOURCE_FILE__ __LINE__ "Failed to parse sig hash algs")
+  | Correct b -> aux b []
+  | Error z   -> Error(AD_decode_error, perror __SOURCE_FILE__ __LINE__ "Failed to parse sig hash algs")
 
-// TODO : replace "bytes" by either DH or ECDH parameters
-type keyShareEntry = namedGroup * b:bytes { repr_bytes (length b) <= 2 }
 
-val keyShareEntryBytes: keyShareEntry -> Tot bytes
-let keyShareEntryBytes (ng, bytes) =
-  let ng_bytes = namedGroupBytes ng in
-  ng_bytes @| vlbytes 2 bytes
+// TODO: replace "bytes" by either DH or ECDH parameters
+type keyShareEntry = namedGroup * b:bytes{repr_bytes (length b) <= 2}
 
-val parseKeyShareEntry: pinverse_t keyShareEntryBytes
-let parseKeyShareEntry b =
-  if length b >= 2 then
-    let ng, key_exchange = split b 2 in
-    match parseNamedGroup ng with
-    | Correct(ng) ->
-	(match vlparse 2 key_exchange with
-	| Correct(ke) -> Correct (ng, ke)
-	| Error(z) -> Error(AD_decode_error, perror __SOURCE_FILE__ __LINE__ "Failed to parse key share entry"))
-    | Error(z) -> Error(z)
-  else Error (AD_decode_error, perror __SOURCE_FILE__ __LINE__ "Too few bytes to parse key share entry")
+type clientKeyShare = l:list keyShareEntry{List.Tot.length l < 65536/4}
 
-val keyShareEntriesBytes: list keyShareEntry -> Tot bytes
-let keyShareEntriesBytes kses =
-  admit(); //TODO
-  vlbytes 2 (List.Tot.fold_left (fun l s -> l @| keyShareEntryBytes s) empty_bytes kses)
-
-val parseKeyShareEntries: pinverse_t keyShareEntriesBytes
-let parseKeyShareEntries b =
-  let rec (aux: b:bytes -> list keyShareEntry -> Tot (result (list keyShareEntry)) (decreases(length b))) = fun b entries ->
-    if length b > 0 then
-      if length b >= 4 then
-	let (ng, data) = split b 2 in
-	match vlsplit 2 data with
-	| Correct(kex, bytes) ->
-	    (match parseKeyShareEntry (ng @| vlbytes 2 kex) with
-	    | Correct(entry) -> aux bytes (entry::entries)
-	    | Error(z) -> Error(z))
-	| Error(z) -> Error(AD_decode_error, perror __SOURCE_FILE__ __LINE__ "Failed to parse key share entry")
-      else Error (AD_decode_error, perror __SOURCE_FILE__ __LINE__ "Too few bytes to parse key share entries")
-    else Correct(entries) in
-  match vlparse 2 b with
-  | Correct (b) ->  aux b []
-  | Error(z) -> Error(AD_decode_error, perror __SOURCE_FILE__ __LINE__ "Failed to parse key share entries")
-  
-type clientKeyShare = l:list keyShareEntry{List.Tot.length l >= 4 /\ List.Tot.length l < 65536}
 type serverKeyShare = keyShareEntry
 
 type keyShare =
   | ClientKeyShare of clientKeyShare
   | ServerKeyShare of serverKeyShare
 
-val clientKeyShareBytes: clientKeyShare -> Tot bytes
-let clientKeyShareBytes cks =
-  keyShareEntriesBytes cks
+val keyShareEntryBytes: keyShareEntry -> Tot (b:bytes{4 <= length b})
+let keyShareEntryBytes (ng, b) =
+  let ng_bytes = namedGroupBytes ng in
+  ng_bytes @| vlbytes 2 b
 
-//val parseClientKeyShare: pinverse_t clientKeyShareBytes
-let parseClientKeyShare b = parseKeyShareEntries b
+val parseKeyShareEntry: pinverse_t keyShareEntryBytes
+let parseKeyShareEntry b =
+  let ng,key_exchange = split b 2 in
+  match parseNamedGroup ng with
+  | Correct ng ->
+    begin
+    match vlparse 2 key_exchange with
+    | Correct ke -> Correct (ng, ke)
+    | Error z    -> Error(AD_decode_error, perror __SOURCE_FILE__ __LINE__ "Failed to parse key share entry")
+    end
+  | Error z -> Error z
 
-val serverKeyShareBytes: serverKeyShare -> Tot bytes
+val inverse_keyShareEntry: x:_ -> Lemma
+  (requires (True))
+  (ensures lemma_inverse_g_f keyShareEntryBytes parseKeyShareEntry x)
+  [SMTPat (parseKeyShareEntry (keyShareEntryBytes x))]
+let inverse_keyShareEntry (ng, x) =
+  let b = namedGroupBytes ng @| vlbytes 2 x in
+  let b0,b1 = split b 2 in
+  let vl,b = split b1 2 in
+  vlparse_vlbytes 2 b;
+  assert (Seq.equal vl (bytes_of_int 2 (length b)));
+  assert (Seq.equal b0 (namedGroupBytes ng));
+  assert (Seq.equal b x)
+
+val pinverse_keyShareEntry: x:_ -> Lemma
+  (requires (True))
+  (ensures lemma_pinverse_f_g Seq.equal keyShareEntryBytes parseKeyShareEntry x)
+  [SMTPat (keyShareEntryBytes (Correct._0 (parseKeyShareEntry x)))]
+let pinverse_keyShareEntry x = ()
+
+// Choice: truncate when maximum length is exceeded
+// Non top-level let rec yields stack overflow during extraction
+let rec keyShareEntriesBytes_aux (b:bytes{length b < 65536}) (kes:list keyShareEntry): Tot (b:bytes{length b < 65536}) (decreases kes) =
+  match kes with
+  | [] -> b
+  | ke::kes ->
+    let b' = b @| keyShareEntryBytes ke in
+    if length b' < 65536 then
+      keyShareEntriesBytes_aux b' kes
+    else b
+
+val keyShareEntriesBytes: list keyShareEntry -> Tot (b:bytes{2 <= length b /\ length b < 65538})
+let keyShareEntriesBytes kes =
+  let b = keyShareEntriesBytes_aux empty_bytes kes in
+  lemma_repr_bytes_values (length b);
+  vlbytes 2 b
+  
+val parseKeyShareEntries: pinverse_t keyShareEntriesBytes
+let parseKeyShareEntries b =
+  let rec (aux: b:bytes -> list keyShareEntry -> Tot (result (list keyShareEntry)) (decreases (length b))) = fun b entries ->
+    if length b > 0 then
+      if length b >= 4 then
+	let ng, data = split b 2 in
+	match vlsplit 2 data with
+	| Correct(kex, bytes) ->
+	  begin
+	  match parseKeyShareEntry (ng @| vlbytes 2 kex) with
+	  | Correct entry -> aux bytes (entry::entries)
+	  | Error z -> Error z
+	  end
+	| Error z -> Error(AD_decode_error, perror __SOURCE_FILE__ __LINE__ "Failed to parse key share entry")
+      else Error (AD_decode_error, perror __SOURCE_FILE__ __LINE__ "Too few bytes to parse key share entries")
+    else Correct entries in
+  match vlparse 2 b with
+  | Correct b -> aux b []
+  | Error z   -> Error(AD_decode_error, perror __SOURCE_FILE__ __LINE__ "Failed to parse key share entries")
+
+val clientKeyShareBytes: clientKeyShare -> Tot (b:bytes{ 2 <= length b /\ length b < 65538 })
+let clientKeyShareBytes cks = keyShareEntriesBytes cks
+
+val parseClientKeyShare: b:bytes{ 2 <= length b /\ length b < 65538 }
+  -> Tot (result clientKeyShare)
+let parseClientKeyShare b =
+  match parseKeyShareEntries b with
+  | Correct kes ->
+    if List.Tot.length kes < 65536/4
+    then Correct kes
+    else Error(AD_decode_error, perror __SOURCE_FILE__ __LINE__ "Failed to parse client key share entries")
+  | Error z -> Error z
+
+val serverKeyShareBytes: serverKeyShare -> Tot (b:bytes{ 4 <= length b })
 let serverKeyShareBytes sks = keyShareEntryBytes sks
 
 val parseServerKeyShare: pinverse_t serverKeyShareBytes
@@ -1275,32 +1452,57 @@ let keyShareBytes = function
   | ClientKeyShare cks -> clientKeyShareBytes cks
   | ServerKeyShare sks -> serverKeyShareBytes sks
 
-(* TODO: FIXME *)
+val parseKeyShare: bool -> bytes -> Tot (result keyShare)
 let parseKeyShare is_client b =
-  if is_client then 
-    match parseClientKeyShare b with
-    | Correct kse -> Correct (ClientKeyShare kse)
-    | Error z -> Error z
+  if is_client then
+    begin
+    if 2 <= length b && length b < 65538 then
+      begin
+      match parseClientKeyShare b with
+      | Correct kse -> Correct (ClientKeyShare kse)
+      | Error z -> Error z
+      end
+    else Error(AD_decode_error, perror __SOURCE_FILE__ __LINE__ "Failed to parse key share")
+    end
   else
-    match parseServerKeyShare b with
-    | Correct ks -> Correct (ServerKeyShare ks)
-    | Error z -> Error z
+    if 4 <= length b then
+      begin
+      match parseServerKeyShare b with
+      | Correct ks -> Correct (ServerKeyShare ks)
+      | Error z -> Error z
+      end
+    else Error(AD_decode_error, perror __SOURCE_FILE__ __LINE__ "Failed to parse key share")
 
 // TODO : give more precise type
-type pskIdentity = b:bytes{length b < 65536}
+type pskIdentity = b:bytes{repr_bytes (length b) <= 2}
 
-val pskIdentityBytes: pskIdentity -> Tot bytes
+val pskIdentityBytes: pskIdentity -> Tot (b:bytes{length b >= 2})
 let pskIdentityBytes pski =
-  lemma_repr_bytes_values (length pski);
-  vlbytes 2 (pski)
+  vlbytes 2 pski
 
-//val parsePskIdentity: pinverse_t pskIdentityBytes
-let parsePskIdentity b = vlparse 2 b
+val parsePskIdentity: pinverse_t pskIdentityBytes
+let parsePskIdentity b =
+  match vlparse 2 b with
+  | Correct vlb -> Correct vlb
+  | Error z -> Error(AD_decode_error, perror __SOURCE_FILE__ __LINE__ "Failed to parse psk_identity")
 
-val pskIdentitiesBytes: list pskIdentity -> Tot bytes
-let pskIdentitiesBytes l =
-  admit(); // TODO
-  vlbytes 2 (List.Tot.fold_left (fun l s -> l @| pskIdentityBytes s) empty_bytes l)
+
+// Choice: truncate when maximum length is exceeded
+// Non top-level let rec yields stack overflow during extraction
+let rec pskIdentitiesBytes_aux (b:bytes{length b < 65536}) (ids:list pskIdentity): Tot (b:bytes{length b < 65536}) (decreases ids) =
+  match ids with
+  | [] -> b
+  | id::ids ->
+    let b' = b @| pskIdentityBytes id in
+    if length b' < 65536 then
+      pskIdentitiesBytes_aux b' ids
+    else b
+
+val pskIdentitiesBytes: list pskIdentity -> Tot (b:bytes{2 <= length b /\ length b < 65538})
+let pskIdentitiesBytes ids =
+  let b = pskIdentitiesBytes_aux empty_bytes ids in
+  lemma_repr_bytes_values (length b);
+  vlbytes 2 b
 
 val parsePskIdentities: pinverse_t pskIdentitiesBytes
 let parsePskIdentities b =
@@ -1310,38 +1512,48 @@ let parsePskIdentities b =
 	let len, data = split b 2 in
 	let len = int_of_bytes len in
 	if length b >= len then
-	  let pski, bytes = split b len in
-	  match parsePskIdentity pski with
-	  | Correct(id) ->
-              admit(); // TODO
-              aux bytes (id::ids)
-	  | Error(z) -> Error(z)
+	  let pski,bytes = split b len in
+	  if length pski >= 2 then
+   	    match parsePskIdentity pski with
+   	    | Correct id -> aux bytes (id::ids)
+   	    | Error z -> Error z
+	  else Error(AD_decode_error, perror __SOURCE_FILE__ __LINE__ "Failed to parse psk identity length")
         else Error(AD_decode_error, perror __SOURCE_FILE__ __LINE__ "Failed to parse psk identity length")
       else Error(AD_decode_error, perror __SOURCE_FILE__ __LINE__ "Expected psk identity to be at least 2 bytes long")
-    else Correct(ids) in
+    else Correct ids in
   match vlparse 2 b with
-  | Correct (b) -> aux b []
-  | Error(z) -> Error(AD_decode_error, perror __SOURCE_FILE__ __LINE__ "Failed to parse psk identities")
+  | Correct b -> aux b []
+  | Error z   -> Error(AD_decode_error, perror __SOURCE_FILE__ __LINE__ "Failed to parse psk identities")
 
-type clientPreSharedKey = l:list pskIdentity{List.Tot.length l >= 2 /\ List.Tot.length l < 65536 }
+type clientPreSharedKey = l:list pskIdentity{List.Tot.length l >= 1 /\ List.Tot.length l < 65536/2}
+
 type serverPreSharedKey = pskIdentity
+
 type preSharedKey =
   | ClientPreSharedKey of clientPreSharedKey
   | ServerPreSharedKey of serverPreSharedKey
 
-val clientPreSharedKeyBytes: clientPreSharedKey -> Tot bytes
+val clientPreSharedKeyBytes: clientPreSharedKey -> Tot (b:bytes{ 2 <= length b /\ length b < 65538 })
 let clientPreSharedKeyBytes cpsk = pskIdentitiesBytes cpsk
 
-//val parseClientPreSharedKey: pinverse_t clientPreSharedKeyBytes
-let parseClientPreSharedKey b = parsePskIdentities b
-
-val serverPreSharedKeyBytes: serverPreSharedKey -> Tot bytes
+val parseClientPreSharedKey: b:bytes{ 2 <= length b /\ length b < 65538 }
+  -> Tot (result clientPreSharedKey)
+let parseClientPreSharedKey b = 
+  match parsePskIdentities b with
+  | Correct ids ->
+    let l = List.Tot.length ids in
+    if 1 <= l && l < 65536/2 
+    then Correct ids
+    else Error(AD_decode_error, perror __SOURCE_FILE__ __LINE__ "Failed to parse client psk identities")
+  | Error z -> Error z
+  
+val serverPreSharedKeyBytes: serverPreSharedKey -> Tot (b:bytes{ 2 <= length b })
 let serverPreSharedKeyBytes cpsk = pskIdentityBytes cpsk
 
-//val parseServerPreSharedKey: pinverse_t serverPreSharedKeyBytes
+val parseServerPreSharedKey: pinverse_t serverPreSharedKeyBytes
 let parseServerPreSharedKey b = parsePskIdentity b
 
-val preSharedKeyBytes: preSharedKey -> Tot bytes
+val preSharedKeyBytes: preSharedKey -> Tot (b:bytes{length b >= 2})
 let preSharedKeyBytes = function
   | ClientPreSharedKey cpsk -> clientPreSharedKeyBytes cpsk
   | ServerPreSharedKey spsk -> serverPreSharedKeyBytes spsk
@@ -1349,15 +1561,24 @@ let preSharedKeyBytes = function
 val parsePreSharedKey: pinverse_t preSharedKeyBytes
 let parsePreSharedKey b =
   match vlparse 2 b with
-  | Correct(b') ->
-      (match vlparse 2 b with
-      | Correct(b'') -> // Client case
-	(match parseClientPreSharedKey b with
-	| Correct(psks) -> admit(); //TODO
-                          Correct(ClientPreSharedKey psks)
-	| Error(z) -> Error(z))
-      | Error(_) -> // Server case
-	(match parseServerPreSharedKey b with
-	| Correct(psk) -> Correct (ServerPreSharedKey psk)
-	| Error(z) -> Error(z)))
-  | Error(z) -> Error(AD_decode_error, perror __SOURCE_FILE__ __LINE__ "Failed to parse pre shared key")
+  | Correct b' ->
+    begin
+      match vlparse 2 b with
+      | Correct b'' -> // Client case
+	begin
+	if length b >= 2 && length b < 65538 then
+	  begin
+	  match parseClientPreSharedKey b with
+	  | Correct psks -> Correct (ClientPreSharedKey psks)
+	  | Error z -> Error z
+	  end
+	else Error(AD_decode_error, perror __SOURCE_FILE__ __LINE__ "Failed to parse  psk")
+	end
+      | Error _ -> // Server case
+	begin
+	match parseServerPreSharedKey b with
+	| Correct psk -> Correct (ServerPreSharedKey psk)
+	| Error z -> Error z
+	end 
+    end
+  | Error z -> Error(AD_decode_error, perror __SOURCE_FILE__ __LINE__ "Failed to parse pre shared key")
