src/tls/Concrete.fst
@@ -1,4 +1,5 @@
 module IdealFlags
+
 let ideal_Nonce = false  
 let ideal_Sig = false 
 let ideal_PMS = false 
